mechanization/theories/Core/Semantic/PER/Lemmas.v
@@ -6,7 +6,7 @@ From McPTS.Core Require Import Base.
 From McPTS.Core.Semantic Require Import PER.CoreTactics PER.Definitions.
 Import Domain_Notations.
 
-Add Parametric Morphism {P : PtsSig}R0 `(R0_morphism : Proper _ ((@relation_equivalence (domain P)) ==> (@relation_equivalence (domain P))) R0) A ρ A' ρ' : (rel_mod_eval R0 A ρ A' ρ')
+Add Parametric Morphism {P : PtsSig} R0 `(R0_morphism : Proper _ ((@relation_equivalence (domain P)) ==> (@relation_equivalence (domain P))) R0) A ρ A' ρ' : (rel_mod_eval R0 A ρ A' ρ')
     with signature (@relation_equivalence (domain P)) ==> iff as rel_mod_eval_morphism.
 Proof.
   split; intros []; econstructor; try eassumption;
@@ -21,7 +21,7 @@ Proof.
     apply HRR'; eassumption.
 Qed.
 
-Lemma per_bot_sym {P : PtsSig} : forall m n : domain_ne P,
+Lemma per_bot_sym {P : PtsSig} : forall (m n : domain_ne P),
     {{ Dom m ≈ n ∈ per_bot }} ->
     {{ Dom n ≈ m ∈ per_bot }}.
 Proof with solve [eauto].
@@ -33,7 +33,7 @@ Qed.
 #[export]
 Hint Resolve per_bot_sym : mcpts.
 
-Lemma per_bot_trans {P : PtsSig} : forall m n l : domain_ne P,
+Lemma per_bot_trans {P : PtsSig} : forall (m n l : domain_ne P),
     {{ Dom m ≈ n ∈ per_bot }} ->
     {{ Dom n ≈ l ∈ per_bot }} ->
     {{ Dom m ≈ l ∈ per_bot }}.
@@ -56,7 +56,7 @@ Proof.
 Qed.
 
 Lemma var_per_bot {P : PtsSig} : forall {n},
-    {{ Dom !n ≈ !n ∈ @per_bot P }}.
+    {{ Dom !n ≈ !n ∈ (@per_bot P) }}.
 Proof.
   intros ? ?. repeat econstructor.
 Qed.
@@ -64,7 +64,7 @@ Qed.
 #[export]
 Hint Resolve var_per_bot : mcpts.
 
-Lemma per_top_sym {P : PtsSig} : forall m n : domain_nf P,
+Lemma per_top_sym {P : PtsSig} : forall (m n : domain_nf P),
     {{ Dom m ≈ n ∈ per_top }} ->
     {{ Dom n ≈ m ∈ per_top }}.
 Proof with solve [eauto].
@@ -76,7 +76,7 @@ Qed.
 #[export]
 Hint Resolve per_top_sym : mcpts.
 
-Lemma per_top_trans {P : PtsSig} : forall m n l : domain_nf P,
+Lemma per_top_trans {P : PtsSig} : forall (m n l : domain_nf P),
     {{ Dom m ≈ n ∈ per_top }} ->
     {{ Dom n ≈ l ∈ per_top }} ->
     {{ Dom m ≈ l ∈ per_top }}.
@@ -111,7 +111,7 @@ Qed.
 #[export]
 Hint Resolve per_bot_then_per_top : mcpts.
 
-Lemma per_top_typ_sym {P : PtsSig} : forall m n : domain P,
+Lemma per_top_typ_sym {P : PtsSig} : forall (m n : domain P),
     {{ Dom m ≈ n ∈ per_top_typ }} ->
     {{ Dom n ≈ m ∈ per_top_typ }}.
 Proof with solve [eauto].
@@ -123,7 +123,7 @@ Qed.
 #[export]
 Hint Resolve per_top_typ_sym : mcpts.
 
-Lemma per_top_typ_trans {P : PtsSig} : forall m n l : domain P,
+Lemma per_top_typ_trans {P : PtsSig} : forall (m n l : domain P),
     {{ Dom m ≈ n ∈ per_top_typ }} ->
     {{ Dom n ≈ l ∈ per_top_typ }} ->
     {{ Dom m ≈ l ∈ per_top_typ }}.
@@ -145,8 +145,7 @@ Proof.
   - eauto using per_top_typ_trans.
 Qed.
 
-
-Lemma per_ne_sym {P : PtsSig} : forall m n : domain P,
+Lemma per_ne_sym {P : PtsSig} : forall (m n : domain P),
     {{ Dom m ≈ n ∈ per_ne }} ->
     {{ Dom n ≈ m ∈ per_ne }}.
 Proof with mautosolve.
@@ -157,7 +156,7 @@ Qed.
 #[export]
 Hint Resolve per_ne_sym : mcpts.
 
-Lemma per_ne_trans {P : PtsSig} : forall m n l : domain P,
+Lemma per_ne_trans {P : PtsSig} : forall (m n l : domain P),
     {{ Dom m ≈ n ∈ per_ne }} ->
     {{ Dom n ≈ l ∈ per_ne }} ->
     {{ Dom m ≈ l ∈ per_ne }}.
@@ -178,49 +177,29 @@ Proof.
   - eauto using per_ne_trans.
 Qed.
 
-Add Parametric Morphism {P : PtsSig} {pred_P : PredicativeSig P} s (per_sort_rec : forall s', pred_rel P pred_P s' s -> relation (domain P)) : (per_sort_elem_core P pred_P s per_sort_rec)
-    with signature (@relation_equivalence (domain P)) ==> eq ==> eq ==> iff as per_sort_elem_core_morphism_iff.
-Proof with mautosolve.
-  simpl.
-  intros R R' HRR'.
-
-  split; intros Horig; [gen R' | gen R];
-    induction Horig;
-    eauto;
-    try (etransitivity; [symmetry + idtac|]; eassumption);
-    intros;
-    destruct_rel_mod_eval;
-    econstructor; mauto 3.
-  1-3: rewrite <- HRR'; mauto.
-  all: rewrite HRR'; mauto.
-Qed.
-
 Add Parametric Morphism {P : PtsSig} {pred_P : PredicativeSig P} s : (per_sort_elem P pred_P s)
     with signature (@relation_equivalence (domain P)) ==> eq ==> eq ==> iff as per_sort_elem_morphism_iff.
 Proof with mautosolve.
-  simp per_sort_elem.
+  simpl.
   intros R R' HRR'.
-
   split; intros Horig; [gen R' | gen R];
-  
-    induction Horig;
-    eauto;
+    induction Horig using per_sort_elem_ind; basic_per_sort_elem_econstructor; mauto;
     try (etransitivity; [symmetry + idtac|]; eassumption);
     intros;
     destruct_rel_mod_eval;
-    econstructor; mauto 3.
-  1-3: rewrite <- HRR'; mauto.
-  all: rewrite HRR'; mauto.
-Qed.
+    econstructor; mauto.
+  - intros.
+    subst.
+    auto.
+  - split; mauto.
+    intros.
+    subst.
+    auto.
+  - intros; subst; auto.
+  - split; intros; subst; mauto.
 
-
-Add Parametric Morphism {P : PtsSig} {pred_P : PredicativeSig P} s per_sort_rec : (per_sort_elem_core P pred_P s per_sort_rec)
-    with signature (@relation_equivalence (domain P)) ==> (@relation_equivalence (domain P)) as per_sort_elem_core_morphism_relation_equivalence.
-Proof with mautosolve.
-  intros * H ? ?.
-  simpl.
-  rewrite H.
-  reflexivity.
+  Unshelve.
+  all: auto.
 Qed.
 
 Add Parametric Morphism {P : PtsSig} {pred_P : PredicativeSig P} s : (per_sort_elem P pred_P s)
@@ -232,7 +211,7 @@ Proof with mautosolve.
   reflexivity.
 Qed.
 
-Add Parametric Morphism {P : PtsSig} {pred_P : PredicativeSig P} s per_sort_rec A ρ A' ρ' : (rel_typ pred_P s per_sort_rec A ρ A' ρ')
+Add Parametric Morphism {P : PtsSig} {pred_P : PredicativeSig P} s A ρ A' ρ' : (rel_typ pred_P s A ρ A' ρ')
     with signature (@relation_equivalence (domain P)) ==> iff as rel_typ_morphism.
 Proof.
   intros * HRR'.
@@ -240,7 +219,7 @@ Proof.
     [setoid_rewrite <- HRR' | setoid_rewrite HRR']; eassumption.
 Qed.
 
-Lemma domain_app_per {P : PtsSig} : forall (f : domain_ne P) f' a a',
+Lemma domain_app_per {P : PtsSig} : forall (f f' : domain_ne P) a a',
   {{ Dom f ≈ f' ∈ per_bot }} ->
   {{ Dom a ≈ a' ∈ per_top }} ->
   {{ Dom f a ≈ f' a' ∈ per_bot }}.
@@ -282,9 +261,11 @@ Ltac apply_relation_equivalence :=
   rewrite_relation_equivalence_left;
   clear_relation_equivalence.
 
-Lemma per_sort_elem_right_irrel {P : PtsSig} {pred_P : PredicativeSig P} : forall s per_sort_rec R a b R' b',
-    {{ DF a ≈ b ∈ per_sort_elem_core P pred_P s per_sort_rec ↘ R }} ->
-    {{ DF a ≈ b' ∈ per_sort_elem_core P pred_P s per_sort_rec ↘ R' }} ->
+
+
+Lemma per_sort_elem_right_irrel {P : PtsSig} {pred_P : PredicativeSig P} : forall s s' R a b R' b',
+    {{ DF a ≈ b ∈ per_sort_elem P pred_P s ↘ R }} ->
+    {{ DF a ≈ b' ∈ per_sort_elem P pred_P s' ↘ R' }} ->
     (R <~> R').
 Proof with (destruct_rel_mod_eval; destruct_rel_mod_app; functional_eval_rewrite_clear; econstructor; intuition).
   simpl.
@@ -292,325 +273,287 @@ Proof with (destruct_rel_mod_eval; destruct_rel_mod_app; functional_eval_rewrite
   remember a as a' in |- *.
   gen a' b' R'.
 
-  induction Horig ; eapply (per_sort_elem_core_strong_ind P pred_P); mauto.    
-  - intros.
-    subst.
-    dependent destruction H4.
-    assert (proj1 (ord_ax P pred_P s0 s_elem ax_s1_s_elem) = proj1 (ord_ax P pred_P s0 s_elem ax_s1_s_elem1)) by (eapply (pred_irrel P pred_P s0 s_elem); mauto).    
-    rewrite <- H in *.
-    apply_relation_equivalence.
-    reflexivity.
-  - intros.
-    subst.
-    dependent destruction H3.
-    assert (proj1 (ord_ax P pred_P s0 s_elem ax_s1_s_elem) = proj1 (ord_ax P pred_P s0 s_elem ax_s1_s_elem0)) by (eapply (pred_irrel P pred_P s0 s_elem); mauto).    
-    rewrite <- H in *.
-    apply_relation_equivalence.
-    reflexivity.
-  - intros * HMono * Heq HE IH * Heq' Hright.
-    subst.
-    dependent destruction Hright;
-      apply_relation_equivalence.
-    split; intros.
-    + admit.
-    + 
-    
-    admit.
-  - intros.
-    subst.
-    dependent destruction H4.
-    apply_relation_equivalence.
-    admit.
-  - intros; subst.
-    dependent destruction H3.
-    apply_relation_equivalence.
-    reflexivity.
-   
-  (* induction Horig. *)
-  (* - intros. *)
-  (*   subst. *)
-  (*   inversion H1. *)
-  (*   subst.     *)
-    
-  (*   assert (proj1 (ord_ax P pred_P s0 s_elem ax_s1_s_elem) = proj1 (ord_ax P pred_P s0 s_elem ax_s1_s_elem0)) by (eapply (pred_irrel P pred_P s0 s_elem); mauto). *)
-  (*   rewrite <- H in *. *)
-  (*   apply_relation_equivalence. *)
-  (*   reflexivity. *)
-
-  (* - intros * Heq Hright. *)
-  (*   subst.     *)
-  (*   dependent destruction Hright; *)
-  (*     apply_relation_equivalence. *)
-  (*   split; intros. *)
-  (*   + admit. *)
-  (*   + admit. *)
-  (* - intros.     *)
-  (*   subst. *)
-  (*   dependent destruction H1. *)
-  (*   apply_relation_equivalence. *)
-  (*   reflexivity. *)
+  induction Horig using per_sort_elem_ind.
+  - admit.
+  -     
+  
+  induction Horig using per_sort_elem_ind; intros * Heq Hright;
+    subst; basic_invert_per_sort_elem Hright; unfold per_sort;
+    intros;
+    apply_relation_equivalence;
+    try reflexivity.
+  specialize (IHHorig _ _ _ eq_refl equiv_a_a').
+  split; intros.
+  - rename equiv_n_n' into equiv0_n_n'.
+    assert (equiv_n_n' : in_rel n n').
+    {
       
-Admitted.
+    }
+  
+  specialize (IHHorig _ _ _ eq_refl ((proj1 equiv_a_a') )).
+  split; intros.
+  - rename equiv_c_c' into equiv0_c_c'.
+    assert (equiv_c_c' : in_rel c c') by firstorder...
+  - assert (equiv0_c_c' : in_rel0 c c') by firstorder...
+  - assert (point_rel <~> point_rel0) by mauto 3.
+    etransitivity; [apply per_eq_morphism_relation_equivalence3 | apply per_eq_morphism_relation_equivalence1]; eauto.
+    etransitivity; [symmetry |]; intuition.
+Qed.
 
 #[local]
-Ltac per_sort_elem_right_irrel_assert1 :=
+Ltac per_univ_elem_right_irrel_assert1 :=
   match goal with
-  | H1 : {{ DF ^?a ≈ ^?b ∈ per_sort_elem_core ?s ?psr ↘ ?R1 }},
-      H2 : {{ DF ^?a ≈ ^?b' ∈ per_sort_elem ?s ?psr ↘ ?R2 }} |- _ =>
+  | H1 : {{ DF ^?a ≈ ^?b ∈ per_univ_elem ?i ↘ ?R1 }},
+      H2 : {{ DF ^?a ≈ ^?b' ∈ per_univ_elem ?i' ↘ ?R2 }} |- _ =>
       assert_fails (unify R1 R2);
       match goal with
       | H : R1 <~> R2 |- _ => fail 1
       | H : R2 <~> R1 |- _ => fail 1
-      | _ => assert (R1 <~> R2) by (eapply per_sort_elem_right_irrel; [apply H1 | apply H2])
+      | _ => assert (R1 <~> R2) by (eapply per_univ_elem_right_irrel; [apply H1 | apply H2])
       end
   end.
 #[local]
-Ltac per_sort_elem_right_irrel_assert := repeat per_sort_elem_right_irrel_assert1.
+Ltac per_univ_elem_right_irrel_assert := repeat per_univ_elem_right_irrel_assert1.
 
-
-Lemma per_sort_elem_sym {P : PtsSig} {pred_P : PredicativeSig P} : forall s per_sort_rec R a b,
-    {{ DF a ≈ b ∈ per_sort_elem_core P pred_P s per_sort_rec ↘ R }} ->
-    {{ DF b ≈ a ∈ per_sort_elem_core P pred_P s per_sort_rec ↘ R }} /\
+Lemma per_univ_elem_sym : forall i R a b,
+    {{ DF a ≈ b ∈ per_univ_elem i ↘ R }} ->
+    {{ DF b ≈ a ∈ per_univ_elem i ↘ R }} /\
       (forall m m',
           {{ Dom m ≈ m' ∈ R }} ->
           {{ Dom m' ≈ m ∈ R }}).
 Proof with mautosolve.
-  (* simpl. *)
-  (* intros s per_sort_rec R a b Horig.    *)
-    
-  (* apply per_sort_elem_core_strong_ind with (s:=s) (motive:=fun s per_sort_rec R a b => per_sort_elem_core P pred_P s per_sort_rec R b a /\ (forall m m' : domain P, R m m' -> R m' m)); intros; subst. *)
-  (* - split. *)
-  (*   +  *)
-  (*     apply per_sort_elem_core_sort with (ax_s1_s_elem := ax_s1_s_elem). exact per_sort_rec_s1.  auto.  auto. *)
-  (*   + intros.       *)
-  (*     rewrite H0 in *. *)
-  (*     eapply H1 with (A := m) (B := m'); mauto 2. *)
-      
-
-      
-  (*     eapply proj1. *)
-  (*     eapply H1; mauto 2. *)
+  simpl.
+  induction 1 using per_univ_elem_ind; subst.
+  - split.
+    + apply per_univ_elem_core_univ'; firstorder.
+    + intros.
+      rewrite H1 in *.
+      destruct_by_head per_univ.      
+      exists x.
+      eapply proj1.
+      eapply H2.
       
       
-  (* induction 1 using per_sort_elem_core_strong_ind; subst. *)
-  (* - split. *)
-  (*   + apply per_sort_elem_core_sort'; firstorder. *)
-  (*   + intros. *)
-  (*     rewrite H1 in *. *)
-  (*     destruct_by_head (@per_sort P). *)
-  (*     eexists. *)
-  (*     eapply proj1... *)
-
-  (* - destruct_conjs. *)
-  (*   split. *)
-  (*   + basic_per_sort_elem_econstructor; eauto. *)
-  (*     * admit. *)
-  (*     * intros. *)
-  (*     assert (in_rel n' n) by eauto. *)
-  (*     assert (in_rel n n) by (etransitivity; eassumption). *)
-  (*     destruct_all. *)
-  (*     destruct_rel_mod_eval. *)
-  (*     functional_eval_rewrite_clear. *)
-  (*     econstructor; eauto. *)
-  (*     per_sort_elem_right_irrel_assert. *)
-  (*     apply_relation_equivalence. *)
-  (*     (* eassumption *) *)
-  (*     admit. *)
-  (*   + apply_relation_equivalence. *)
-  (*     intros. *)
-  (*     assert (in_rel n' n) by eauto. *)
-  (*     assert (in_rel n n) by (etransitivity; eassumption). *)
-  (*     destruct_rel_mod_eval. *)
-  (*     destruct_rel_mod_app. *)
-  (*     functional_eval_rewrite_clear. *)
-  (*     econstructor; eauto. *)
-  (*     per_sort_elem_right_irrel_assert. *)
-  (*     (* intuition. *) *)
-  (*     admit. *)
+      eapply H2 with (A:= d{{{ 𝕌@j' }}}) (B:= d{{{  𝕌@j' }}}).
       
-  (* - split; [basic_per_sort_elem_econstructor | apply_relation_equivalence]; mauto 3. *)
-Admitted.
-
-
-Corollary per_sort_sym {P : PtsSig} {pred_P : PredicativeSig P} : forall s per_sort_rec R a b,
-    {{ DF a ≈ b ∈ per_sort_elem_core P pred_P s per_sort_rec ↘ R }} ->
-    {{ DF b ≈ a ∈ per_sort_elem_core P pred_P s per_sort_rec ↘ R }}.
-Proof.  
-  intros * ?%per_sort_elem_sym.
-  firstorder.
+      
+      eapply proj1...
+      
+  - split; [basic_per_univ_elem_econstructor | intros; apply_relation_equivalence]...
+  - destruct_conjs.
+    split.
+    + basic_per_univ_elem_econstructor; eauto.
+      intros.
+      assert (in_rel c' c) by eauto.
+      assert (in_rel c c) by (etransitivity; eassumption).
+      destruct_all.
+      destruct_rel_mod_eval.
+      functional_eval_rewrite_clear.
+      econstructor; eauto.
+      per_univ_elem_right_irrel_assert.
+      apply_relation_equivalence.
+      eassumption.
+    + apply_relation_equivalence.
+      intros.
+      assert (in_rel c' c) by eauto.
+      assert (in_rel c c) by (etransitivity; eassumption).
+      destruct_rel_mod_eval.
+      destruct_rel_mod_app.
+      functional_eval_rewrite_clear.
+      econstructor; eauto.
+      per_univ_elem_right_irrel_assert.
+      intuition.
+  - destruct_conjs.
+    split; [basic_per_univ_elem_econstructor | apply_relation_equivalence]; mauto 3.
+    apply_relation_equivalence.
+    etransitivity; [apply per_eq_morphism_relation_equivalence2 | apply per_eq_morphism_relation_equivalence3]; mauto 3.
+  - split; [econstructor | intros; apply_relation_equivalence]...
 Qed.
 
-Corollary per_sort_sym' {P : PtsSig} {pred_P : PredicativeSig P} : forall s a b,
-    {{ Dom a ≈ b ∈ per_sort pred_P s }} ->
-    {{ Dom b ≈ a ∈ per_sort pred_P s }}.
+Corollary per_univ_sym : forall i R a b,
+    {{ DF a ≈ b ∈ per_univ_elem i ↘ R }} ->
+    {{ DF b ≈ a ∈ per_univ_elem i ↘ R }}.
 Proof.
-  intros * [? ?%per_sort_elem_sym].
+  intros * ?%per_univ_elem_sym.
   firstorder.
 Qed.
 
-Corollary per_elem_sym {P : PtsSig} {pred_P : PredicativeSig P} : forall s R a b m m',
-    {{ DF a ≈ b ∈ per_sort_elem P pred_P s ↘ R }} ->
+Corollary per_univ_sym' : forall i a b,
+    {{ Dom a ≈ b ∈ per_univ i }} ->
+    {{ Dom b ≈ a ∈ per_univ i }}.
+Proof.
+  intros * [? ?%per_univ_elem_sym].
+  firstorder.
+Qed.
+
+Corollary per_elem_sym : forall i R a b m m',
+    {{ DF a ≈ b ∈ per_univ_elem i ↘ R }} ->
     {{ Dom m ≈ m' ∈ R }} ->
     {{ Dom m' ≈ m ∈ R }}.
 Proof.
-  intros * ?%per_sort_elem_sym.
+  intros * ?%per_univ_elem_sym.
   firstorder.
 Qed.
 
-Corollary per_sort_elem_left_irrel {P : PtsSig} {pred_P : PredicativeSig P} : forall s s' R a b R' a',
-    {{ DF a ≈ b ∈ per_sort_elem P pred_P s ↘ R }} ->
-    {{ DF a' ≈ b ∈ per_sort_elem P pred_P s' ↘ R' }} ->
+Corollary per_univ_elem_left_irrel : forall i i' R a b R' a',
+    {{ DF a ≈ b ∈ per_univ_elem i ↘ R }} ->
+    {{ DF a' ≈ b ∈ per_univ_elem i' ↘ R' }} ->
     (R <~> R').
 Proof.
-  intros * ?%per_sort_sym ?%per_sort_sym.
-  eauto using per_sort_elem_right_irrel.
+  intros * ?%per_univ_sym ?%per_univ_sym.
+  eauto using per_univ_elem_right_irrel.
 Qed.
 
-Corollary per_sort_elem_cross_irrel {P : PtsSig} {pred_P : PredicativeSig P} : forall s s' R a b R' b',
-    {{ DF a ≈ b ∈ per_sort_elem P pred_P s ↘ R }} ->
-    {{ DF b' ≈ a ∈ per_sort_elem P pred_P s' ↘ R' }} ->
+Corollary per_univ_elem_cross_irrel : forall i i' R a b R' b',
+    {{ DF a ≈ b ∈ per_univ_elem i ↘ R }} ->
+    {{ DF b' ≈ a ∈ per_univ_elem i' ↘ R' }} ->
     (R <~> R').
 Proof.
-  intros * ? ?%per_sort_sym.
-  eauto using per_sort_elem_right_irrel.
+  intros * ? ?%per_univ_sym.
+  eauto using per_univ_elem_right_irrel.
 Qed.
 
-Ltac do_per_sort_elem_irrel_assert1 :=
-  let tactic_error o1 o2 := fail 2 "per_sort_elem_irrel biconditional between" o1 "and" o2 "cannot be solved" in
+Ltac do_per_univ_elem_irrel_assert1 :=
+  let tactic_error o1 o2 := fail 2 "per_univ_elem_irrel biconditional between" o1 "and" o2 "cannot be solved" in
   match goal with
-  | H1 : {{ DF ^?a ≈ ^_ ∈ per_sort_elem ?P ?pred_P ?s ↘ ?R1 }},
-      H2 : {{ DF ^?a ≈ ^_ ∈ per_sort_elem ?P ?pred_P ?s' ↘ ?R2 }} |- _ =>
+  | H1 : {{ DF ^?a ≈ ^_ ∈ per_univ_elem ?i ↘ ?R1 }},
+      H2 : {{ DF ^?a ≈ ^_ ∈ per_univ_elem ?i' ↘ ?R2 }} |- _ =>
       assert_fails (unify R1 R2);
       match goal with
       | H : R1 <~> R2 |- _ => fail 1
       | H : R2 <~> R1 |- _ => fail 1
-      | _ => assert (R1 <~> R2) by (eapply per_sort_elem_right_irrel; [apply H1 | apply H2]) || tactic_error R1 R2
+      | _ => assert (R1 <~> R2) by (eapply per_univ_elem_right_irrel; [apply H1 | apply H2]) || tactic_error R1 R2
       end
-  | H1 : {{ DF ^_ ≈ ^?b ∈ per_sort_elem ?P ?pred_P ?s ↘ ?R1 }},
-      H2 : {{ DF ^_ ≈ ^?b ∈ per_sort_elem ?P ?pred_P ?s' ↘ ?R2 }} |- _ =>
+  | H1 : {{ DF ^_ ≈ ^?b ∈ per_univ_elem ?i ↘ ?R1 }},
+      H2 : {{ DF ^_ ≈ ^?b ∈ per_univ_elem ?i' ↘ ?R2 }} |- _ =>
       assert_fails (unify R1 R2);
       match goal with
       | H : R1 <~> R2 |- _ => fail 1
       | H : R2 <~> R1 |- _ => fail 1
-      | _ => assert (R1 <~> R2) by (eapply per_sort_elem_left_irrel; [apply H1 | apply H2]) || tactic_error R1 R2
+      | _ => assert (R1 <~> R2) by (eapply per_univ_elem_left_irrel; [apply H1 | apply H2]) || tactic_error R1 R2
       end
-  | H1 : {{ DF ^?a ≈ ^_ ∈ per_sort_elem ?P ?pred_P ?s ↘ ?R1 }},
-      H2 : {{ DF ^_ ≈ ^?a ∈ per_sort_elem ?P ?pred_P ?s' ↘ ?R2 }} |- _ =>
+  | H1 : {{ DF ^?a ≈ ^_ ∈ per_univ_elem ?i ↘ ?R1 }},
+      H2 : {{ DF ^_ ≈ ^?a ∈ per_univ_elem ?i' ↘ ?R2 }} |- _ =>
       (** Order matters less here as H1 and H2 cannot be exchanged *)
       assert_fails (unify R1 R2);
       match goal with
       | H : R1 <~> R2 |- _ => fail 1
       | H : R2 <~> R1 |- _ => fail 1
-      | _ => assert (R1 <~> R2) by (eapply per_sort_elem_cross_irrel; [apply H1 | apply H2]) || tactic_error R1 R2
+      | _ => assert (R1 <~> R2) by (eapply per_univ_elem_cross_irrel; [apply H1 | apply H2]) || tactic_error R1 R2
       end
   end.
 
-Ltac do_per_sort_elem_irrel_assert :=
-  repeat do_per_sort_elem_irrel_assert1.
+Ltac do_per_univ_elem_irrel_assert :=
+  repeat do_per_univ_elem_irrel_assert1.
 
-Ltac handle_per_sort_elem_irrel :=
+Ltac handle_per_univ_elem_irrel :=
   functional_eval_rewrite_clear;
-  do_per_sort_elem_irrel_assert;
+  do_per_univ_elem_irrel_assert;
   apply_relation_equivalence;
   clear_dups.
 
-Lemma per_sort_elem_trans {P : PtsSig} {pred_P : PredicativeSig P} : forall s R a1 a2,
-    per_sort_elem P pred_P s R a1 a2 ->
-    (forall s' a3,
-        per_sort_elem P pred_P s' R a2 a3 ->
-        per_sort_elem P pred_P s R a1 a3) /\
+Lemma per_univ_elem_trans : forall i R a1 a2,
+    per_univ_elem i R a1 a2 ->
+    (forall j a3,
+        per_univ_elem j R a2 a3 ->
+        per_univ_elem i R a1 a3) /\
       (forall m1 m2 m3,
           R m1 m2 ->
           R m2 m3 ->
           R m1 m3).
-Proof with (basic_per_sort_elem_econstructor; mautosolve 4).
-  induction 1 using per_sort_elem_ind;
+Proof with (basic_per_univ_elem_econstructor; mautosolve 4).
+  induction 1 using per_univ_elem_ind;
     [> split;
-     [ intros * HT2; basic_invert_per_sort_elem HT2
+     [ intros * HT2; basic_invert_per_univ_elem HT2
      | intros * HTR1 HTR2; apply_relation_equivalence ] ..]; mauto.
-  - subst. mauto.
-  - (* sort case *)
+  - (* univ case *)
     subst.
     destruct HTR1, HTR2.
     functional_eval_rewrite_clear.
-    handle_per_sort_elem_irrel.
+    handle_per_univ_elem_irrel.
     eexists.
     specialize (H2 _ _ _ H0) as [].
     intuition.
+  - (* nat case *)
+    idtac...
   - (* pi case *)
     destruct_conjs.
-    basic_per_sort_elem_econstructor; eauto.
-    + handle_per_sort_elem_irrel.
+    basic_per_univ_elem_econstructor; eauto.
+    + handle_per_univ_elem_irrel.
       intuition.
-      admit.
     + intros.
-      handle_per_sort_elem_irrel.
-      assert (in_rel n n') by (firstorder; admit).
-      assert (in_rel n n) by intuition.
-      assert (in_rel0 n n) by (intuition; admit).
+      handle_per_univ_elem_irrel.
+      assert (in_rel c c') by firstorder.
+      assert (in_rel c c) by intuition.
+      assert (in_rel0 c c) by intuition.
       destruct_rel_mod_eval.
       functional_eval_rewrite_clear.
-      (* handle_per_sort_elem_irrel... *)
-      admit.
+      handle_per_univ_elem_irrel...
   - (* fun case *)
     intros.
-    assert (in_rel n n) by intuition.
+    assert (in_rel c c) by intuition.
     destruct_rel_mod_eval.
     destruct_rel_mod_app.
-    handle_per_sort_elem_irrel.
+    handle_per_univ_elem_irrel.
     econstructor; eauto.
     intuition.
+  - (* eq case *)
+    destruct_conjs.
+    handle_per_univ_elem_irrel.
+    basic_per_univ_elem_econstructor; intuition.
+    bulky_rewrite1.
+    reflexivity.
   - (* neut case *)
     idtac...
-Admitted.
+Qed.
 
-Corollary per_sort_trans {P : PtsSig} {pred_P : PredicativeSig P} : forall s s' R a1 a2 a3,
-    per_sort_elem P pred_P s R a1 a2 ->
-    per_sort_elem P pred_P s' R a2 a3 ->
-    per_sort_elem P pred_P s R a1 a3.
+Corollary per_univ_trans : forall i j R a1 a2 a3,
+    per_univ_elem i R a1 a2 ->
+    per_univ_elem j R a2 a3 ->
+    per_univ_elem i R a1 a3.
 Proof.
-  intros * ?%per_sort_elem_trans.
+  intros * ?%per_univ_elem_trans.
   firstorder.
 Qed.
 
-Corollary per_sort_trans' {P : PtsSig} {pred_P : PredicativeSig P} : forall s s' a1 a2 a3,
-    {{ Dom a1 ≈ a2 ∈ per_sort pred_P s }} ->
-    {{ Dom a2 ≈ a3 ∈ per_sort pred_P s' }} ->
-    {{ Dom a1 ≈ a3 ∈ per_sort pred_P s }}.
+Corollary per_univ_trans' : forall i j a1 a2 a3,
+    {{ Dom a1 ≈ a2 ∈ per_univ i }} ->
+    {{ Dom a2 ≈ a3 ∈ per_univ j }} ->
+    {{ Dom a1 ≈ a3 ∈ per_univ i }}.
 Proof.
   intros * [? ?] [? ?].
-  handle_per_sort_elem_irrel.
-  firstorder mauto using per_sort_trans.
+  handle_per_univ_elem_irrel.
+  firstorder mauto using per_univ_trans.
 Qed.
 
-Corollary per_elem_trans {P : PtsSig} {pred_P : PredicativeSig P} : forall s R a1 a2 m1 m2 m3,
-    per_sort_elem P pred_P s R a1 a2 ->
+Corollary per_elem_trans : forall i R a1 a2 m1 m2 m3,
+    per_univ_elem i R a1 a2 ->
     R m1 m2 ->
     R m2 m3 ->
     R m1 m3.
 Proof.
-  intros * ?% per_sort_elem_trans.
+  intros * ?% per_univ_elem_trans.
   firstorder.
 Qed.
 
 #[export]
-Instance per_sort_PER {P : PtsSig} {pred_P : PredicativeSig P} {s R} : PER (per_sort_elem P pred_P s R).
+Instance per_univ_PER {i R} : PER (per_univ_elem i R).
 Proof.
   split.
-  - auto using per_sort_sym.
-  - eauto using per_sort_trans.
+  - auto using per_univ_sym.
+  - eauto using per_univ_trans.
 Qed.
 
 #[export]
-Instance per_sort_PER' {P : PtsSig} {pred_P : PredicativeSig P} {s} : PER (per_sort pred_P s).
+Instance per_univ_PER' {i} : PER (per_univ i).
 Proof.
   split.
-  - auto using per_sort_sym'.
-  - eauto using per_sort_trans'.
+  - auto using per_univ_sym'.
+  - eauto using per_univ_trans'.
 Qed.
 
 #[export]
-Instance per_elem_PER {P : PtsSig} {pred_P : PredicativeSig P} {s R a b} `(H : per_sort_elem P pred_P s R a b) : PER R.
+Instance per_elem_PER {i R a b} `(H : per_univ_elem i R a b) : PER R.
 Proof.
   split.
   - pose proof (fun m m' => per_elem_sym _ _ _ _ m m' H). eauto.
@@ -618,234 +561,283 @@ Proof.
 Qed.
 
 (** These lemmas get rid of the unnecessary PER premises. *)
-Lemma per_sort_elem_pi' {P : PtsSig} {pred_P : PredicativeSig P} :
-  forall s_in s_out s (r : Ru P s_in s_out s) a a' ρ B ρ' B'
-    (in_rel : relation (domain P))
-    (out_rel : forall {c c'} (equiv_c_c' : {{ Dom c ≈ c' ∈ in_rel }}), relation (domain P))
+Lemma per_univ_elem_pi' :
+  forall i a a' ρ B ρ' B'
+    (in_rel : relation domain)
+    (out_rel : forall {c c'} (equiv_c_c' : {{ Dom c ≈ c' ∈ in_rel }}), relation domain)
     elem_rel,
-    {{ DF a ≈ a' ∈ per_sort_elem P pred_P s_in ↘ in_rel}} ->
+    {{ DF a ≈ a' ∈ per_univ_elem i ↘ in_rel}} ->
     (forall {c c'} (equiv_c_c' : {{ Dom c ≈ c' ∈ in_rel }}),
-        rel_mod_eval (per_sort_elem P pred_P s_out) B d{{{ ρ ↦ c }}} B' d{{{ ρ' ↦ c' }}} (out_rel equiv_c_c')) ->
+        rel_mod_eval (per_univ_elem i) B d{{{ ρ ↦ c }}} B' d{{{ ρ' ↦ c' }}} (out_rel equiv_c_c')) ->
     (elem_rel <~> fun f f' => forall c c' (equiv_c_c' : {{ Dom c ≈ c' ∈ in_rel }}), rel_mod_app f c f' c' (out_rel equiv_c_c')) ->
-    {{ DF Π r a ρ B ≈ Π r a' ρ' B' ∈ per_sort_elem P pred_P s ↘ elem_rel }}.
+    {{ DF Π a ρ B ≈ Π a' ρ' B' ∈ per_univ_elem i ↘ elem_rel }}.
 Proof.
   intros.
-  basic_per_sort_elem_econstructor; eauto.
-  (* typeclasses eauto. *)
-  admit.
-Admitted.
+  basic_per_univ_elem_econstructor; eauto.
+  typeclasses eauto.
+Qed.
+
+Lemma per_univ_elem_eq' :
+  forall (i : nat) {a a' m1 m1' m2 m2' : domain} (point_rel elem_rel : relation domain),
+    {{ DF a ≈ a' ∈ per_univ_elem i ↘ point_rel }} ->
+    {{ Dom m1 ≈ m1' ∈ point_rel }} ->
+    {{ Dom m2 ≈ m2' ∈ point_rel }} ->
+    elem_rel <~> per_eq point_rel m1 m2' ->
+    {{ DF Eq a m1 m2 ≈ Eq a' m1' m2' ∈ per_univ_elem i ↘ elem_rel }}.
+Proof.
+  intros.
+  basic_per_univ_elem_econstructor; eauto.
+  typeclasses eauto.
+Qed.
 
 
-Ltac per_sort_elem_econstructor :=
-  (repeat intro; hnf; (eapply per_sort_elem_pi')) + basic_per_sort_elem_econstructor.
+Ltac per_univ_elem_econstructor :=
+  (repeat intro; hnf; (eapply per_univ_elem_pi' || eapply per_univ_elem_eq')) + basic_per_univ_elem_econstructor.
 
 #[export]
-Hint Resolve per_sort_elem_pi' : mcpts.
+Hint Resolve per_univ_elem_pi' per_univ_elem_eq' : mcpts.
 
-Lemma per_sort_elem_pi_clean_inversion {P : PtsSig} {pred_P : PredicativeSig P} : forall {s_in s_out s} {r : Ru P s_in s_out s} {a a' in_rel ρ ρ' B B' elem_rel},
-    {{ DF a ≈ a' ∈ per_sort_elem P pred_P s_in ↘ in_rel }} ->
-    {{ DF Π r a ρ B ≈ Π r a' ρ' B' ∈ per_sort_elem P pred_P s ↘ elem_rel }} ->
-    exists (out_rel : forall {n n'} (equiv_n_n' : {{ Dom n ≈ n' ∈ in_rel }}), relation (domain P)),
-      (forall n n' (equiv_n_n' : {{ Dom n ≈ n' ∈ in_rel }}),
-          rel_mod_eval (per_sort_elem P pred_P s_out) B d{{{ ρ ↦ n }}} B' d{{{ ρ' ↦ n' }}} (out_rel equiv_n_n')) /\
-        (elem_rel <~> fun f f' => forall n n' (equiv_n_n' : {{ Dom n ≈ n' ∈ in_rel }}), rel_mod_app f n f' n' (out_rel equiv_n_n')).
+Lemma per_univ_elem_pi_clean_inversion : forall {i j a a' in_rel ρ ρ' B B' elem_rel},
+    {{ DF a ≈ a' ∈ per_univ_elem i ↘ in_rel }} ->
+    {{ DF Π a ρ B ≈ Π a' ρ' B' ∈ per_univ_elem j ↘ elem_rel }} ->
+    exists (out_rel : forall {c c'} (equiv_c_c' : {{ Dom c ≈ c' ∈ in_rel }}), relation domain),
+      (forall c c' (equiv_c_c' : {{ Dom c ≈ c' ∈ in_rel }}),
+          rel_mod_eval (per_univ_elem j) B d{{{ ρ ↦ c }}} B' d{{{ ρ' ↦ c' }}} (out_rel equiv_c_c')) /\
+        (elem_rel <~> fun f f' => forall c c' (equiv_c_c' : {{ Dom c ≈ c' ∈ in_rel }}), rel_mod_app f c f' c' (out_rel equiv_c_c')).
 Proof.
   intros * Ha HΠ.
-  basic_invert_per_sort_elem HΠ.
-  handle_per_sort_elem_irrel.
+  basic_invert_per_univ_elem HΠ.
+  handle_per_univ_elem_irrel.
   eexists.
   split.
-  - instantiate (1 := fun n n' (equiv_n_n' : in_rel n n') m m' =>
+  - instantiate (1 := fun c c' (equiv_c_c' : in_rel c c') m m' =>
                         forall R,
-                          rel_typ pred_P s_out B d{{{ ρ ↦ n }}} B' d{{{ ρ' ↦ n' }}} R ->
+                          rel_typ j B d{{{ ρ ↦ c }}} B' d{{{ ρ' ↦ c' }}} R ->
                           R m m').
     intros.
-    (* assert (in_rel0 n n') by intuition. *)
-    (* (on_all_hyp: destruct_rel_by_assumption in_rel0). *)
-    (* econstructor; eauto. *)
-    (* apply -> per_sort_elem_morphism_iff; eauto. *)
-    (* split; intuition. *)
-    (* destruct_by_head rel_typ. *)
-    (* handle_per_sort_elem_irrel. *)
-    (* intuition. *)
-    admit.
-  - (* split; intros; *)
-    (*   [assert (in_rel0 n n') by intuition; (on_all_hyp: destruct_rel_by_assumption in_rel0) *)
-    (*   | assert (in_rel n n') by intuition; (on_all_hyp: destruct_rel_by_assumption in_rel)]; *)
-    (*   econstructor; intuition. *)
-    (* destruct_by_head rel_typ. *)
-    (* handle_per_sort_elem_irrel. *)
-    (* intuition. *)
-    admit.
-Admitted.
+    assert (in_rel0 c c') by intuition.
+    (on_all_hyp: destruct_rel_by_assumption in_rel0).
+    econstructor; eauto.
+    apply -> per_univ_elem_morphism_iff; eauto.
+    split; intuition.
+    destruct_by_head rel_typ.
+    handle_per_univ_elem_irrel.
+    intuition.
+  - split; intros;
+      [assert (in_rel0 c c') by intuition; (on_all_hyp: destruct_rel_by_assumption in_rel0)
+      | assert (in_rel c c') by intuition; (on_all_hyp: destruct_rel_by_assumption in_rel)];
+      econstructor; intuition.
+    destruct_by_head rel_typ.
+    handle_per_univ_elem_irrel.
+    intuition.
+Qed.
 
-Ltac invert_per_sort_elem H :=
-  (unshelve eapply (per_sort_elem_pi_clean_inversion _) in H; shelve_unifiable; [eassumption |]; destruct H as [? []])
-  + basic_invert_per_sort_elem H.
+Ltac invert_per_univ_elem H :=
+  (unshelve eapply (per_univ_elem_pi_clean_inversion _) in H; shelve_unifiable; [eassumption |]; destruct H as [? []])
+  + basic_invert_per_univ_elem H.
 
-Ltac invert_per_sort_elems := match_by_head per_sort_elem ltac:(fun H => directed invert_per_sort_elem H).
+Ltac invert_per_univ_elems := match_by_head per_univ_elem ltac:(fun H => directed invert_per_univ_elem H).
 
+Lemma per_univ_elem_cumu : forall i a0 a1 R,
+    {{ DF a0 ≈ a1 ∈ per_univ_elem i ↘ R }} ->
+    {{ DF a0 ≈ a1 ∈ per_univ_elem (S i) ↘ R }}.
+Proof with solve [eauto].
+  simpl.
+  induction 1 using per_univ_elem_ind; subst;
+    per_univ_elem_econstructor; eauto.
+  intros.
+  destruct_rel_mod_eval.
+  econstructor...
+Qed.
 
-(* These are all lemmas about subtyping.  We might need to replace them with something else *)
+#[export]
+Hint Resolve per_univ_elem_cumu : mcpts.
 
-(* Lemma per_subtyp_to_sort_elem : forall a b i, *)
-(*     {{ Sub a <: b at i }} -> *)
-(*     exists R R', *)
-(*       {{ DF a ≈ a ∈ per_sort_elem i ↘ R }} /\ *)
-(*         {{ DF b ≈ b ∈ per_sort_elem i ↘ R' }}. *)
-(* Proof. *)
-(*   destruct 1; do 2 eexists; mauto; *)
-(*     split; *)
-(*     try (etransitivity; try eassumption; symmetry; eassumption); *)
-(*     per_sort_elem_econstructor; mauto 3; *)
-(*     try apply Equivalence_Reflexive. *)
+Lemma per_univ_elem_cumu_ge : forall i i' a0 a1 R,
+    i <= i' ->
+    {{ DF a0 ≈ a1 ∈ per_univ_elem i ↘ R }} ->
+    {{ DF a0 ≈ a1 ∈ per_univ_elem i' ↘ R }}.
+Proof with mautosolve.
+  induction 1...
+Qed.
 
-(*   lia. *)
-(* Qed. *)
+#[export]
+Hint Resolve per_univ_elem_cumu_ge : mcpts.
 
-(* Lemma per_elem_subtyping : forall A B i, *)
-(*     {{ Sub A <: B at i }} -> *)
-(*     forall R R' a b, *)
-(*       {{ DF A ≈ A ∈ per_sort_elem i ↘ R }} -> *)
-(*       {{ DF B ≈ B ∈ per_sort_elem i ↘ R' }} -> *)
-(*       R a b -> *)
-(*       R' a b. *)
-(* Proof. *)
-(*   induction 1; intros; *)
-(*     handle_per_sort_elem_irrel; *)
-(*     saturate_refl; *)
-(*     invert_per_sort_elems; *)
-(*     handle_per_sort_elem_irrel; *)
-(*     clear_refl_eqs; *)
-(*     trivial. *)
-(*   - firstorder mauto. *)
-(*   - intros. *)
-(*     handle_per_sort_elem_irrel. *)
-(*     destruct_rel_mod_eval. *)
-(*     saturate_refl_for per_sort_elem. *)
-(*     destruct_rel_mod_app. *)
-(*     simplify_evals. *)
-(*     econstructor; eauto. *)
-(*     intuition. *)
-(* Qed. *)
+Lemma per_univ_elem_cumu_max_left : forall i j a0 a1 R,
+    {{ DF a0 ≈ a1 ∈ per_univ_elem i ↘ R }} ->
+    {{ DF a0 ≈ a1 ∈ per_univ_elem (max i j) ↘ R }}.
+Proof with mautosolve.
+  intros.
+  assert (i <= max i j) by lia...
+Qed.
 
-(* Lemma per_elem_subtyping_gen : forall a b i a' b' R R' m n, *)
-(*     {{ Sub a <: b at i }} -> *)
-(*     {{ DF a ≈ a' ∈ per_sort_elem i ↘ R }} -> *)
-(*     {{ DF b ≈ b' ∈ per_sort_elem i ↘ R' }} -> *)
-(*     R m n -> *)
-(*     R' m n. *)
-(* Proof. *)
-(*   intros. *)
-(*   eapply per_elem_subtyping; saturate_refl; try eassumption. *)
-(* Qed. *)
+Lemma per_univ_elem_cumu_max_right : forall i j a0 a1 R,
+    {{ DF a0 ≈ a1 ∈ per_univ_elem j ↘ R }} ->
+    {{ DF a0 ≈ a1 ∈ per_univ_elem (max i j) ↘ R }}.
+Proof with mautosolve.
+  intros.
+  assert (j <= max i j) by lia...
+Qed.
 
-(* Lemma per_subtyp_refl1 : forall a b i R, *)
-(*     {{ DF a ≈ b ∈ per_sort_elem i ↘ R }} -> *)
-(*     {{ Sub a <: b at i }}. *)
-(* Proof. *)
-(*   simpl; induction 1 using per_sort_elem_ind; *)
-(*     subst; *)
-(*     mauto; *)
-(*     destruct_all. *)
-(*     assert ({{ DF Π a ρ B ≈ Π a' ρ' B' ∈ per_sort_elem i ↘ elem_rel }}) *)
-(*       by (per_sort_elem_econstructor; intuition; destruct_rel_mod_eval; mauto). *)
-(*     saturate_refl_for per_sort_elem. *)
-(*     econstructor; eauto. *)
-(*     intros; *)
-(*       destruct_rel_mod_eval; *)
-(*       functional_eval_rewrite_clear; *)
-(*       trivial. *)
-(* Qed. *)
+Lemma per_subtyp_to_univ_elem : forall a b i,
+    {{ Sub a <: b at i }} ->
+    exists R R',
+      {{ DF a ≈ a ∈ per_univ_elem i ↘ R }} /\
+        {{ DF b ≈ b ∈ per_univ_elem i ↘ R' }}.
+Proof.
+  destruct 1; do 2 eexists; mauto;
+    split;
+    try (etransitivity; try eassumption; symmetry; eassumption);
+    per_univ_elem_econstructor; mauto 3;
+    try apply Equivalence_Reflexive.
 
-(* #[export] *)
-(* Hint Resolve per_subtyp_refl1 : mcpts. *)
+  lia.
+Qed.
 
-(* Lemma per_subtyp_refl2 : forall a b i R, *)
-(*     {{ DF a ≈ b ∈ per_sort_elem i ↘ R }} -> *)
-(*     {{ Sub b <: a at i }}. *)
-(* Proof. *)
-(*   intros. *)
-(*   symmetry in H. *)
-(*   eauto using per_subtyp_refl1. *)
-(* Qed. *)
+Lemma per_elem_subtyping : forall A B i,
+    {{ Sub A <: B at i }} ->
+    forall R R' a b,
+      {{ DF A ≈ A ∈ per_univ_elem i ↘ R }} ->
+      {{ DF B ≈ B ∈ per_univ_elem i ↘ R' }} ->
+      R a b ->
+      R' a b.
+Proof.
+  induction 1; intros;
+    handle_per_univ_elem_irrel;
+    saturate_refl;
+    invert_per_univ_elems;
+    handle_per_univ_elem_irrel;
+    clear_refl_eqs;
+    trivial.
+  - firstorder mauto.
+  - intros.
+    handle_per_univ_elem_irrel.
+    destruct_rel_mod_eval.
+    saturate_refl_for per_univ_elem.
+    destruct_rel_mod_app.
+    simplify_evals.
+    econstructor; eauto.
+    intuition.
+Qed.
 
-(* #[export] *)
-(* Hint Resolve per_subtyp_refl2 : mcpts. *)
+Lemma per_elem_subtyping_gen : forall a b i a' b' R R' m n,
+    {{ Sub a <: b at i }} ->
+    {{ DF a ≈ a' ∈ per_univ_elem i ↘ R }} ->
+    {{ DF b ≈ b' ∈ per_univ_elem i ↘ R' }} ->
+    R m n ->
+    R' m n.
+Proof.
+  intros.
+  eapply per_elem_subtyping; saturate_refl; try eassumption.
+Qed.
 
-(* Lemma per_subtyp_trans : forall a1 a2 i, *)
-(*     {{ Sub a1 <: a2 at i }} -> *)
-(*     forall a3, *)
-(*       {{ Sub a2 <: a3 at i }} -> *)
-(*       {{ Sub a1 <: a3 at i }}. *)
-(* Proof. *)
-(*   induction 1; intros ? Hsub; simpl in *. *)
-(*   1,2,5: progressive_inversion; mauto. *)
-(*   - econstructor; lia. *)
-(*   - dependent destruction Hsub. *)
-(*     handle_per_sort_elem_irrel. *)
-(*     econstructor; eauto. *)
-(*     + etransitivity; eassumption. *)
-(*     + intros. *)
-(*       invert_per_sort_elems. *)
-(*       handle_per_sort_elem_irrel. *)
-(*       saturate_refl_for in_rel1. *)
-(*       destruct_rel_mod_eval. *)
-(*       intuition. *)
-(*   - dependent destruction Hsub. *)
-(*     handle_per_sort_elem_irrel. *)
-(*     econstructor; etransitivity; eauto. *)
-(* Qed. *)
+Lemma per_subtyp_refl1 : forall a b i R,
+    {{ DF a ≈ b ∈ per_univ_elem i ↘ R }} ->
+    {{ Sub a <: b at i }}.
+Proof.
+  simpl; induction 1 using per_univ_elem_ind;
+    subst;
+    mauto;
+    destruct_all.
+    assert ({{ DF Π a ρ B ≈ Π a' ρ' B' ∈ per_univ_elem i ↘ elem_rel }})
+      by (per_univ_elem_econstructor; intuition; destruct_rel_mod_eval; mauto).
+    saturate_refl_for per_univ_elem.
+    econstructor; eauto.
+    intros;
+      destruct_rel_mod_eval;
+      functional_eval_rewrite_clear;
+      trivial.
+Qed.
 
-(* #[export] *)
-(* Hint Resolve per_subtyp_trans : mcpts. *)
+#[export]
+Hint Resolve per_subtyp_refl1 : mcpts.
 
-(* #[export] *)
-(* Instance per_subtyp_trans_ins i : Transitive (per_subtyp i). *)
-(* Proof. *)
-(*   eauto using per_subtyp_trans. *)
-(* Qed. *)
+Lemma per_subtyp_refl2 : forall a b i R,
+    {{ DF a ≈ b ∈ per_univ_elem i ↘ R }} ->
+    {{ Sub b <: a at i }}.
+Proof.
+  intros.
+  symmetry in H.
+  eauto using per_subtyp_refl1.
+Qed.
 
-(* Lemma per_subtyp_transp : forall a b i a' b' R R', *)
-(*     {{ Sub a <: b at i }} -> *)
-(*     {{ DF a ≈ a' ∈ per_sort_elem i ↘ R }} -> *)
-(*     {{ DF b ≈ b' ∈ per_sort_elem i ↘ R' }} -> *)
-(*     {{ Sub a' <: b' at i }}. *)
-(* Proof. *)
-(*   mauto using per_subtyp_refl1, per_subtyp_refl2. *)
-(* Qed. *)
+#[export]
+Hint Resolve per_subtyp_refl2 : mcpts.
 
-(* Lemma per_subtyp_cumu : forall a1 a2 i, *)
-(*     {{ Sub a1 <: a2 at i }} -> *)
-(*     forall j, *)
-(*       i <= j -> *)
-(*       {{ Sub a1 <: a2 at j }}. *)
-(* Proof. *)
-(*   induction 1; intros; econstructor; mauto. *)
-(*   lia. *)
-(* Qed. *)
+Lemma per_subtyp_trans : forall a1 a2 i,
+    {{ Sub a1 <: a2 at i }} ->
+    forall a3,
+      {{ Sub a2 <: a3 at i }} ->
+      {{ Sub a1 <: a3 at i }}.
+Proof.
+  induction 1; intros ? Hsub; simpl in *.
+  1,2,5: progressive_inversion; mauto.
+  - econstructor; lia.
+  - dependent destruction Hsub.
+    handle_per_univ_elem_irrel.
+    econstructor; eauto.
+    + etransitivity; eassumption.
+    + intros.
+      invert_per_univ_elems.
+      handle_per_univ_elem_irrel.
+      saturate_refl_for in_rel1.
+      destruct_rel_mod_eval.
+      intuition.
+  - dependent destruction Hsub.
+    handle_per_univ_elem_irrel.
+    econstructor; etransitivity; eauto.
+Qed.
 
-(* #[export] *)
-(* Hint Resolve per_subtyp_cumu : mcpts. *)
+#[export]
+Hint Resolve per_subtyp_trans : mcpts.
 
-(* Lemma per_subtyp_cumu_left : forall a1 a2 i j, *)
-(*     {{ Sub a1 <: a2 at i }} -> *)
-(*     {{ Sub a1 <: a2 at max i j }}. *)
-(* Proof. *)
-(*   intros. eapply per_subtyp_cumu; try eassumption. *)
-(*   lia. *)
-(* Qed. *)
+#[export]
+Instance per_subtyp_trans_ins i : Transitive (per_subtyp i).
+Proof.
+  eauto using per_subtyp_trans.
+Qed.
 
-(* Lemma per_subtyp_cumu_right : forall a1 a2 i j, *)
-(*     {{ Sub a1 <: a2 at i }} -> *)
-(*     {{ Sub a1 <: a2 at max j i }}. *)
-(* Proof. *)
-(*   intros. eapply per_subtyp_cumu; try eassumption. *)
-(*   lia. *)
-(* Qed. *)
+Lemma per_subtyp_transp : forall a b i a' b' R R',
+    {{ Sub a <: b at i }} ->
+    {{ DF a ≈ a' ∈ per_univ_elem i ↘ R }} ->
+    {{ DF b ≈ b' ∈ per_univ_elem i ↘ R' }} ->
+    {{ Sub a' <: b' at i }}.
+Proof.
+  mauto using per_subtyp_refl1, per_subtyp_refl2.
+Qed.
 
-Add Parametric Morphism {P : PtsSig} {pred_P : PredicativeSig P} : (@per_ctx_env P pred_P)
-    with signature (@relation_equivalence (env P)) ==> eq ==> eq ==> iff as per_ctx_env_morphism_iff.
+Lemma per_subtyp_cumu : forall a1 a2 i,
+    {{ Sub a1 <: a2 at i }} ->
+    forall j,
+      i <= j ->
+      {{ Sub a1 <: a2 at j }}.
+Proof.
+  induction 1; intros; econstructor; mauto.
+  lia.
+Qed.
+
+#[export]
+Hint Resolve per_subtyp_cumu : mcpts.
+
+Lemma per_subtyp_cumu_left : forall a1 a2 i j,
+    {{ Sub a1 <: a2 at i }} ->
+    {{ Sub a1 <: a2 at max i j }}.
+Proof.
+  intros. eapply per_subtyp_cumu; try eassumption.
+  lia.
+Qed.
+
+Lemma per_subtyp_cumu_right : forall a1 a2 i j,
+    {{ Sub a1 <: a2 at i }} ->
+    {{ Sub a1 <: a2 at max j i }}.
+Proof.
+  intros. eapply per_subtyp_cumu; try eassumption.
+  lia.
+Qed.
+
+Add Parametric Morphism : per_ctx_env
+    with signature (@relation_equivalence env) ==> eq ==> eq ==> iff as per_ctx_env_morphism_iff.
 Proof with mautosolve.
   intros R R' HRR'.
   split; intro Horig; [gen R' | gen R];
@@ -853,8 +845,8 @@ Proof with mautosolve.
     apply_relation_equivalence; try reflexivity...
 Qed.
 
-Add Parametric Morphism {P : PtsSig} {pred_P : PredicativeSig P} : (@per_ctx_env P pred_P)
-    with signature (@relation_equivalence (env P)) ==> (@relation_equivalence (ctx P)) as per_ctx_env_morphism_relation_equivalence.
+Add Parametric Morphism : per_ctx_env
+    with signature (@relation_equivalence env) ==> (@relation_equivalence ctx) as per_ctx_env_morphism_relation_equivalence.
 Proof.
   intros * HRR' Γ Γ'.
   simpl.
@@ -862,11 +854,11 @@ Proof.
   reflexivity.
 Qed.
 
-Lemma per_ctx_env_right_irrel {P : PtsSig} {pred_P : PredicativeSig P} : forall Γ Δ Δ' R R',
-    {{ DF Γ ≈ Δ ∈ (@per_ctx_env P pred_P) ↘ R }} ->
-    {{ DF Γ ≈ Δ' ∈ (@per_ctx_env P pred_P) ↘ R' }} ->
+Lemma per_ctx_env_right_irrel : forall Γ Δ Δ' R R',
+    {{ DF Γ ≈ Δ ∈ per_ctx_env ↘ R }} ->
+    {{ DF Γ ≈ Δ' ∈ per_ctx_env ↘ R' }} ->
     R <~> R'.
-Proof with (destruct_rel_typ; handle_per_sort_elem_irrel; eexists; intuition).
+Proof with (destruct_rel_typ; handle_per_univ_elem_irrel; eexists; intuition).
   intros * Horig; gen Δ' R'.
   induction Horig; intros * Hright;
     inversion Hright; subst;
@@ -876,45 +868,43 @@ Proof with (destruct_rel_typ; handle_per_sort_elem_irrel; eexists; intuition).
   intros ρ ρ'.
   split; intros Hcons; dependent destruction Hcons.
   - assert {{ Dom ρ ↯ ≈ ρ' ↯ ∈ tail_rel0 }} by intuition...
-    admit.
   - assert {{ Dom ρ ↯ ≈ ρ' ↯ ∈ tail_rel }} by intuition...
-    admit.
-Admitted.
+Qed.
 
-Lemma per_ctx_env_sym {P : PtsSig} {pred_P : PredicativeSig P} : forall Γ Δ R,
-    {{ DF Γ ≈ Δ ∈ @per_ctx_env P pred_P ↘ R }} ->
-    {{ DF Δ ≈ Γ ∈ @per_ctx_env P pred_P ↘ R }} /\
+Lemma per_ctx_env_sym : forall Γ Δ R,
+    {{ DF Γ ≈ Δ ∈ per_ctx_env ↘ R }} ->
+    {{ DF Δ ≈ Γ ∈ per_ctx_env ↘ R }} /\
       (forall ρ ρ',
           {{ Dom ρ ≈ ρ' ∈ R }} ->
           {{ Dom ρ' ≈ ρ ∈ R }}).
 Proof with solve [intuition].
   simpl.
-  (* induction 1; split; simpl in *; destruct_conjs; try econstructor; intuition; *)
-  (*   pose proof (@relation_equivalence_pointwise env). *)
-  (* - assert (tail_rel ρ' ρ) by eauto. *)
-  (*   assert (tail_rel ρ ρ) by (etransitivity; eassumption). *)
-  (*   destruct_rel_mod_eval. *)
-  (*   handle_per_sort_elem_irrel. *)
-  (*   econstructor; eauto. *)
-  (*   symmetry... *)
-  (* - apply_relation_equivalence. *)
-  (*   destruct_by_head cons_per_ctx_env. *)
-  (*   assert (tail_rel d{{{ ρ' ↯ }}} d{{{ ρ ↯ }}}) by eauto. *)
-  (*   assert (tail_rel d{{{ ρ ↯ }}} d{{{ ρ ↯ }}}) by (etransitivity; eassumption). *)
-  (*   destruct_rel_mod_eval. *)
-  (*   eexists; symmetry; handle_per_sort_elem_irrel; intuition. *)
-Admitted.
+  induction 1; split; simpl in *; destruct_conjs; try econstructor; intuition;
+    pose proof (@relation_equivalence_pointwise env).
+  - assert (tail_rel ρ' ρ) by eauto.
+    assert (tail_rel ρ ρ) by (etransitivity; eassumption).
+    destruct_rel_mod_eval.
+    handle_per_univ_elem_irrel.
+    econstructor; eauto.
+    symmetry...
+  - apply_relation_equivalence.
+    destruct_by_head cons_per_ctx_env.
+    assert (tail_rel d{{{ ρ' ↯ }}} d{{{ ρ ↯ }}}) by eauto.
+    assert (tail_rel d{{{ ρ ↯ }}} d{{{ ρ ↯ }}}) by (etransitivity; eassumption).
+    destruct_rel_mod_eval.
+    eexists; symmetry; handle_per_univ_elem_irrel; intuition.
+Qed.
 
-Corollary per_ctx_sym {P : PtsSig} {pred_P : PredicativeSig P} : forall Γ Δ R,
-    {{ DF Γ ≈ Δ ∈ @per_ctx_env P pred_P ↘ R }} ->
-    {{ DF Δ ≈ Γ ∈ @per_ctx_env P pred_P ↘ R }}.
+Corollary per_ctx_sym : forall Γ Δ R,
+    {{ DF Γ ≈ Δ ∈ per_ctx_env ↘ R }} ->
+    {{ DF Δ ≈ Γ ∈ per_ctx_env ↘ R }}.
 Proof.
   intros * ?%per_ctx_env_sym.
   firstorder.
 Qed.
 
-Corollary per_env_sym {P : PtsSig} {pred_P : PredicativeSig P} : forall Γ Δ R ρ ρ',
-    {{ DF Γ ≈ Δ ∈ @per_ctx_env P pred_P ↘ R }} ->
+Corollary per_env_sym : forall Γ Δ R ρ ρ',
+    {{ DF Γ ≈ Δ ∈ per_ctx_env ↘ R }} ->
     {{ Dom ρ ≈ ρ' ∈ R }} ->
     {{ Dom ρ' ≈ ρ ∈ R }}.
 Proof.
@@ -922,18 +912,18 @@ Proof.
   firstorder.
 Qed.
 
-Corollary per_ctx_env_left_irrel {P : PtsSig} {pred_P : PredicativeSig P} : forall Γ Γ' Δ R R',
-    {{ DF Γ ≈ Δ ∈ @per_ctx_env P pred_P ↘ R }} ->
-    {{ DF Γ' ≈ Δ ∈ @per_ctx_env P pred_P ↘ R' }} ->
+Corollary per_ctx_env_left_irrel : forall Γ Γ' Δ R R',
+    {{ DF Γ ≈ Δ ∈ per_ctx_env ↘ R }} ->
+    {{ DF Γ' ≈ Δ ∈ per_ctx_env ↘ R' }} ->
     R <~> R'.
 Proof.
   intros * ?%per_ctx_sym ?%per_ctx_sym.
   eauto using per_ctx_env_right_irrel.
 Qed.
 
-Corollary per_ctx_env_cross_irrel {P : PtsSig} {pred_P : PredicativeSig P} : forall Γ Δ Δ' R R',
-    {{ DF Γ ≈ Δ ∈ @per_ctx_env P pred_P ↘ R }} ->
-    {{ DF Δ' ≈ Γ ∈ @per_ctx_env P pred_P ↘ R' }} ->
+Corollary per_ctx_env_cross_irrel : forall Γ Δ Δ' R R',
+    {{ DF Γ ≈ Δ ∈ per_ctx_env ↘ R }} ->
+    {{ DF Δ' ≈ Γ ∈ per_ctx_env ↘ R' }} ->
     R <~> R'.
 Proof.
   intros * ? ?%per_ctx_sym.
@@ -979,54 +969,54 @@ Ltac handle_per_ctx_env_irrel :=
   apply_relation_equivalence;
   clear_dups.
 
-Lemma per_ctx_env_trans {P : PtsSig} {pred_P : PredicativeSig P} : forall Γ1 Γ2 R,
-    {{ DF Γ1 ≈ Γ2 ∈ @per_ctx_env P pred_P ↘ R }} ->
+Lemma per_ctx_env_trans : forall Γ1 Γ2 R,
+    {{ DF Γ1 ≈ Γ2 ∈ per_ctx_env ↘ R }} ->
     (forall Γ3,
-        {{ DF Γ2 ≈ Γ3 ∈ @per_ctx_env P pred_P ↘ R }} ->
-        {{ DF Γ1 ≈ Γ3 ∈ @per_ctx_env P pred_P ↘ R }}) /\
+        {{ DF Γ2 ≈ Γ3 ∈ per_ctx_env ↘ R }} ->
+        {{ DF Γ1 ≈ Γ3 ∈ per_ctx_env ↘ R }}) /\
       (forall ρ1 ρ2 ρ3,
           {{ Dom ρ1 ≈ ρ2 ∈ R }} ->
           {{ Dom ρ2 ≈ ρ3 ∈ R }} ->
           {{ Dom ρ1 ≈ ρ3 ∈ R }}).
-Proof with solve [eauto using per_sort_trans].
+Proof with solve [eauto using per_univ_trans].
   simpl.
-  (* induction 1; subst; *)
-  (*   [> split; *)
-  (*    [ inversion 1; subst; eauto *)
-  (*    | intros; destruct_conjs; eauto] ..]; *)
-  (*   pose proof (@relation_equivalence_pointwise env); *)
-  (*   handle_per_ctx_env_irrel; *)
-  (*   try solve [intuition]. *)
-  (* - econstructor; only 4: reflexivity; eauto. *)
-  (*   + apply_relation_equivalence. intuition. *)
-  (*   + intros. *)
-  (*     assert (tail_rel ρ ρ) by intuition. *)
-  (*     assert (tail_rel0 ρ ρ') by intuition. *)
-  (*     destruct_rel_typ. *)
-  (*     handle_per_sort_elem_irrel. *)
-  (*     econstructor; intuition. *)
-  (*     (** This one cannot be replaced with `etransitivity` as we need different `i`s. *) *)
-  (*     eapply per_sort_trans; [| eassumption]; eassumption. *)
-  (* - destruct_by_head cons_per_ctx_env. *)
-  (*   assert (tail_rel d{{{ ρ ↯ }}} d{{{ ρ' ↯ }}}) by eauto. *)
-  (*   destruct_rel_typ. *)
-  (*   handle_per_sort_elem_irrel. *)
-  (*   eexists. *)
-  (*   apply_relation_equivalence. *)
-  (*   etransitivity; intuition. *)
-Admitted.
+  induction 1; subst;
+    [> split;
+     [ inversion 1; subst; eauto
+     | intros; destruct_conjs; eauto] ..];
+    pose proof (@relation_equivalence_pointwise env);
+    handle_per_ctx_env_irrel;
+    try solve [intuition].
+  - econstructor; only 4: reflexivity; eauto.
+    + apply_relation_equivalence. intuition.
+    + intros.
+      assert (tail_rel ρ ρ) by intuition.
+      assert (tail_rel0 ρ ρ') by intuition.
+      destruct_rel_typ.
+      handle_per_univ_elem_irrel.
+      econstructor; intuition.
+      (** This one cannot be replaced with `etransitivity` as we need different `i`s. *)
+      eapply per_univ_trans; [| eassumption]; eassumption.
+  - destruct_by_head cons_per_ctx_env.
+    assert (tail_rel d{{{ ρ ↯ }}} d{{{ ρ' ↯ }}}) by eauto.
+    destruct_rel_typ.
+    handle_per_univ_elem_irrel.
+    eexists.
+    apply_relation_equivalence.
+    etransitivity; intuition.
+Qed.
 
-Corollary per_ctx_trans {P : PtsSig} {pred_P : PredicativeSig P} : forall Γ1 Γ2 Γ3 R,
-    {{ DF Γ1 ≈ Γ2 ∈ @per_ctx_env P pred_P ↘ R }} ->
-    {{ DF Γ2 ≈ Γ3 ∈ @per_ctx_env P pred_P ↘ R }} ->
-    {{ DF Γ1 ≈ Γ3 ∈ @per_ctx_env P pred_P ↘ R }}.
+Corollary per_ctx_trans : forall Γ1 Γ2 Γ3 R,
+    {{ DF Γ1 ≈ Γ2 ∈ per_ctx_env ↘ R }} ->
+    {{ DF Γ2 ≈ Γ3 ∈ per_ctx_env ↘ R }} ->
+    {{ DF Γ1 ≈ Γ3 ∈ per_ctx_env ↘ R }}.
 Proof.
   intros * ?% per_ctx_env_trans.
   firstorder.
 Qed.
 
-Corollary per_env_trans {P : PtsSig} {pred_P : PredicativeSig P} : forall Γ1 Γ2 R ρ1 ρ2 ρ3,
-    {{ DF Γ1 ≈ Γ2 ∈ @per_ctx_env P pred_P ↘ R }} ->
+Corollary per_env_trans : forall Γ1 Γ2 R ρ1 ρ2 ρ3,
+    {{ DF Γ1 ≈ Γ2 ∈ per_ctx_env ↘ R }} ->
     {{ Dom ρ1 ≈ ρ2 ∈ R }} ->
     {{ Dom ρ2 ≈ ρ3 ∈ R }} ->
     {{ Dom ρ1 ≈ ρ3 ∈ R }}.
@@ -1036,7 +1026,7 @@ Proof.
 Qed.
 
 #[export]
-Instance per_ctx_PER {P : PtsSig} {pred_P : PredicativeSig P} {R} : PER (@per_ctx_env P pred_P R).
+Instance per_ctx_PER {R} : PER (per_ctx_env R).
 Proof.
   split.
   - auto using per_ctx_sym.
@@ -1044,7 +1034,7 @@ Proof.
 Qed.
 
 #[export]
-Instance per_env_PER {P : PtsSig} {pred_P : PredicativeSig P} {R Γ Δ} (H : @per_ctx_env P pred_P R Γ Δ) : PER R.
+Instance per_env_PER {R Γ Δ} (H : per_ctx_env R Γ Δ) : PER R.
 Proof.
   split.
   - pose proof (fun ρ ρ' => per_env_sym _ _ _ ρ ρ' H); auto.
@@ -1052,14 +1042,14 @@ Proof.
 Qed.
 
 (** This lemma removes the PER argument *)
-Lemma per_ctx_env_cons' {P : PtsSig} {pred_P : PredicativeSig P} : forall {Γ Γ' s A A' tail_rel}
-                             (head_rel : forall {ρ ρ'} (equiv_ρ_ρ' : {{ Dom ρ ≈ ρ' ∈ tail_rel }}), relation (domain P))
+Lemma per_ctx_env_cons' : forall {Γ Γ' i A A' tail_rel}
+                             (head_rel : forall {ρ ρ'} (equiv_ρ_ρ' : {{ Dom ρ ≈ ρ' ∈ tail_rel }}), relation domain)
                              env_rel,
-    {{ EF Γ ≈ Γ' ∈ @per_ctx_env P pred_P ↘ tail_rel }} ->
+    {{ EF Γ ≈ Γ' ∈ per_ctx_env ↘ tail_rel }} ->
     (forall {ρ ρ'} (equiv_ρ_ρ' : {{ Dom ρ ≈ ρ' ∈ tail_rel }}),
-        rel_typ pred_P s A ρ A' ρ' (head_rel equiv_ρ_ρ')) ->
+        rel_typ i A ρ A' ρ' (head_rel equiv_ρ_ρ')) ->
     (env_rel <~> cons_per_ctx_env tail_rel (@head_rel)) ->
-    {{ EF Γ, A::Sort@s ≈ Γ', A'::Sort@s ∈ @per_ctx_env P pred_P ↘ env_rel }}.
+    {{ EF Γ, A ≈ Γ', A' ∈ per_ctx_env ↘ env_rel }}.
 Proof.
   intros.
   econstructor; eauto.
@@ -1072,39 +1062,39 @@ Hint Resolve per_ctx_env_cons' : mcpts.
 Ltac per_ctx_env_econstructor :=
   (repeat intro; hnf; eapply per_ctx_env_cons') + econstructor.
 
-Lemma per_ctx_env_cons_clean_inversion {P : PtsSig} {pred_P : PredicativeSig P} : forall {Γ Γ' env_relΓ A A' env_relΓA s},
-    {{ EF Γ ≈ Γ' ∈ @per_ctx_env P pred_P ↘ env_relΓ }} ->
-    {{ EF Γ, A::Sort@s ≈ Γ', A'::Sort@s ∈ @per_ctx_env P pred_P ↘ env_relΓA }} -> 
-    exists (head_rel : forall {ρ ρ'} (equiv_ρ_ρ' : {{ Dom ρ ≈ ρ' ∈ env_relΓ }}), relation (domain P)),
+Lemma per_ctx_env_cons_clean_inversion : forall {Γ Γ' env_relΓ A A' env_relΓA},
+    {{ EF Γ ≈ Γ' ∈ per_ctx_env ↘ env_relΓ }} ->
+    {{ EF Γ, A ≈ Γ', A' ∈ per_ctx_env ↘ env_relΓA }} -> 
+    exists i (head_rel : forall {ρ ρ'} (equiv_ρ_ρ' : {{ Dom ρ ≈ ρ' ∈ env_relΓ }}), relation domain),
       (forall ρ ρ' (equiv_ρ_ρ' : {{ Dom ρ ≈ ρ' ∈ env_relΓ }}),
-          rel_typ pred_P s A ρ A' ρ' (head_rel equiv_ρ_ρ')) /\
+          rel_typ i A ρ A' ρ' (head_rel equiv_ρ_ρ')) /\
         (env_relΓA <~> cons_per_ctx_env env_relΓ (@head_rel)).
 Proof with intuition.
   intros * HΓ HΓA.
   inversion HΓA; subst.
   handle_per_ctx_env_irrel.
   eexists.
+  eexists.
   split; intros.
   - instantiate (1 := fun ρ ρ' (equiv_ρ_ρ' : env_relΓ ρ ρ') m m' =>
                         forall R,
-                          rel_typ pred_P s A ρ A' ρ' R ->
+                          rel_typ i A ρ A' ρ' R ->
                           {{ Dom m ≈ m' ∈ R }}).
     assert (tail_rel ρ ρ') by intuition.
     (on_all_hyp: destruct_rel_by_assumption tail_rel).
     econstructor; eauto.
-    apply -> per_sort_elem_morphism_iff; eauto.
+    apply -> per_univ_elem_morphism_iff; eauto.
     split; intros...
-    destruct_by_head (@rel_typ P).
-    handle_per_sort_elem_irrel...
+    destruct_by_head rel_typ.
+    handle_per_univ_elem_irrel...
   - intros ρ ρ'.
-    split; intros; destruct_by_head (@cons_per_ctx_env P);
+    split; intros; destruct_by_head cons_per_ctx_env;
       assert {{ Dom ρ ↯ ≈ ρ' ↯ ∈ tail_rel }} by intuition;
       (on_all_hyp: destruct_rel_by_assumption tail_rel);
       unshelve eexists; intros...
-    destruct_by_head (@rel_typ P).
-    handle_per_sort_elem_irrel...
-    
-Admitted.
+    destruct_by_head rel_typ.
+    handle_per_univ_elem_irrel...
+Qed.
 
 Ltac invert_per_ctx_env H :=
   (unshelve eapply (per_ctx_env_cons_clean_inversion _) in H; [eassumption | |]; deex_in H; destruct H as [])
@@ -1114,111 +1104,1354 @@ Ltac invert_per_ctx_envs := match_by_head per_ctx_env ltac:(fun H => directed in
 
 Ltac invert_per_ctx_envs_of rel := match_by_head (per_ctx_env rel) ltac:(fun H => directed invert_per_ctx_env H).
 
-Lemma per_ctx_respects_length {P : PtsSig} {pred_P : PredicativeSig P} : forall {Γ Γ'},
-    {{ Exp Γ ≈ Γ' ∈ @per_ctx P pred_P }} ->
+Lemma per_ctx_respects_length : forall {Γ Γ'},
+    {{ Exp Γ ≈ Γ' ∈ per_ctx }} ->
     length Γ = length Γ'.
 Proof.
   intros * [? H].
   induction H; simpl; congruence.
 Qed.
 
-(* The remaining lemmas are about context subtyping.  We might need to replace them at some point *)
+Lemma per_ctx_subtyp_to_env : forall Γ Δ,
+    {{ SubE Γ <: Δ }} ->
+    exists R R',
+      {{ EF Γ ≈ Γ ∈ per_ctx_env ↘ R }} /\
+        {{ EF Δ ≈ Δ ∈ per_ctx_env ↘ R' }}.
+Proof.
+  destruct 1; destruct_all.
+  - repeat eexists; econstructor; apply Equivalence_Reflexive.
+  - eauto.
+Qed.
 
-(* Lemma per_ctx_subtyp_to_env : forall Γ Δ, *)
-(*     {{ SubE Γ <: Δ }} -> *)
-(*     exists R R', *)
-(*       {{ EF Γ ≈ Γ ∈ per_ctx_env ↘ R }} /\ *)
-(*         {{ EF Δ ≈ Δ ∈ per_ctx_env ↘ R' }}. *)
+Lemma per_ctx_env_subtyping : forall Γ Δ,
+    {{ SubE Γ <: Δ }} ->
+    forall R R' ρ ρ',
+      {{ EF Γ ≈ Γ ∈ per_ctx_env ↘ R }} ->
+      {{ EF Δ ≈ Δ ∈ per_ctx_env ↘ R' }} ->
+      R ρ ρ' ->
+      R' ρ ρ'.
+Proof.
+  induction 1; intros;
+    handle_per_ctx_env_irrel;
+    invert_per_ctx_envs;
+    apply_relation_equivalence;
+    trivial.
+
+  destruct_by_head cons_per_ctx_env.
+  assert {{ Dom ρ ↯ ≈ ρ' ↯ ∈ tail_rel0 }} by intuition.
+  unshelve eexists; [eassumption |].
+  destruct_rel_typ.
+  eapply per_elem_subtyping with (i := max i1 (max i0 i)); try eassumption.
+  - eauto using per_subtyp_cumu_right.
+  - saturate_refl.
+    eauto using per_univ_elem_cumu_max_left.
+  - saturate_refl.
+    eauto using per_univ_elem_cumu_max_left, per_univ_elem_cumu_max_right.
+Qed.
+
+Lemma per_ctx_subtyp_refl1 : forall Γ Δ R,
+    {{ EF Γ ≈ Δ ∈ per_ctx_env ↘ R }} ->
+    {{ SubE Γ <: Δ }}.
+Proof.
+  induction 1; mauto.
+
+  assert (exists R, {{ EF Γ , A ≈ Γ' , A' ∈ per_ctx_env ↘ R }}) by
+    (eexists; eapply per_ctx_env_cons'; eassumption).
+  destruct_all.
+  econstructor; try solve [saturate_refl; mauto 2].
+  intros.
+  destruct_rel_typ.
+  simplify_evals.
+  eauto using per_subtyp_refl1.
+Qed.
+
+Lemma per_ctx_subtyp_refl2 : forall Γ Δ R,
+    {{ EF Γ ≈ Δ ∈ per_ctx_env ↘ R }} ->
+    {{ SubE Δ <: Γ }}.
+Proof.
+  intros. symmetry in H. eauto using per_ctx_subtyp_refl1.
+Qed.
+
+Lemma per_ctx_subtyp_trans : forall Γ1 Γ2,
+    {{ SubE Γ1 <: Γ2 }} ->
+    forall Γ3,
+      {{ SubE Γ2 <: Γ3 }} ->
+      {{ SubE Γ1 <: Γ3 }}.
+Proof.
+  induction 1; intros;
+    dir_inversion_by_head per_ctx_subtyp; subst;
+    repeat invert_per_ctx_envs;
+    mauto 1; clear_PER.
+
+  handle_per_ctx_env_irrel.
+  econstructor; try eassumption.
+  - firstorder.
+  - instantiate (1 := max i i0).
+    intros.
+    assert {{ Dom ρ ≈ ρ' ∈ tail_rel0 }}
+      by (apply_relation_equivalence; eapply per_ctx_env_subtyping; revgoals; eassumption).
+    saturate_refl_for tail_rel.
+    destruct_rel_typ.
+    handle_per_univ_elem_irrel.
+    etransitivity; intuition mauto using per_subtyp_cumu_left, per_subtyp_cumu_right.
+  - econstructor; intuition.
+    + typeclasses eauto.
+    + solve_refl.
+  - econstructor; mauto 3.
+    + typeclasses eauto.
+    + solve_refl.
+Qed.
+
+#[export]
+Hint Resolve per_ctx_subtyp_trans : mcpts.
+
+#[export]
+Instance per_ctx_subtyp_trans_ins : Transitive per_ctx_subtyp.
+Proof.
+  eauto using per_ctx_subtyp_trans.
+Qed.
+
+
+
+
+
+
+
+
+
+
+
+
+
+
+
+
+
+
+
+
+
+(* From Coq Require Import Equivalence Lia Morphisms Morphisms_Prop Morphisms_Relations PeanoNat Relation_Definitions RelationClasses. *)
+(* From Equations Require Import Equations. *)
+
+(* From McPTS Require Import PtsSignature LibTactics. *)
+(* From McPTS.Core Require Import Base. *)
+(* From McPTS.Core.Semantic Require Import PER.CoreTactics PER.Definitions. *)
+(* Import Domain_Notations. *)
+
+(* Add Parametric Morphism {P : PtsSig}R0 `(R0_morphism : Proper _ ((@relation_equivalence (domain P)) ==> (@relation_equivalence (domain P))) R0) A ρ A' ρ' : (rel_mod_eval R0 A ρ A' ρ') *)
+(*     with signature (@relation_equivalence (domain P)) ==> iff as rel_mod_eval_morphism. *)
 (* Proof. *)
-(*   destruct 1; destruct_all. *)
-(*   - repeat eexists; econstructor; apply Equivalence_Reflexive. *)
-(*   - eauto. *)
+(*   split; intros []; econstructor; try eassumption; *)
+(*     [> eapply R0_morphism; [symmetry + idtac |]; eassumption ..]. *)
 (* Qed. *)
 
-(* Lemma per_ctx_env_subtyping : forall Γ Δ, *)
-(*     {{ SubE Γ <: Δ }} -> *)
-(*     forall R R' ρ ρ', *)
-(*       {{ EF Γ ≈ Γ ∈ per_ctx_env ↘ R }} -> *)
-(*       {{ EF Δ ≈ Δ ∈ per_ctx_env ↘ R' }} -> *)
-(*       R ρ ρ' -> *)
-(*       R' ρ ρ'. *)
+(* Add Parametric Morphism {P : PtsSig} f a f' a' : (rel_mod_app f a f' a') *)
+(*     with signature (@relation_equivalence (domain P)) ==> iff as rel_mod_app_morphism. *)
 (* Proof. *)
-(*   induction 1; intros; *)
-(*     handle_per_ctx_env_irrel; *)
-(*     invert_per_ctx_envs; *)
-(*     apply_relation_equivalence; *)
-(*     trivial. *)
-
-(*   destruct_by_head cons_per_ctx_env. *)
-(*   assert {{ Dom ρ ↯ ≈ ρ' ↯ ∈ tail_rel0 }} by intuition. *)
-(*   unshelve eexists; [eassumption |]. *)
-(*   destruct_rel_typ. *)
-(*   eapply per_elem_subtyping with (i := max i1 (max i0 i)); try eassumption. *)
-(*   - eauto using per_subtyp_cumu_right. *)
-(*   - saturate_refl. *)
-(*     eauto using per_sort_elem_cumu_max_left. *)
-(*   - saturate_refl. *)
-(*     eauto using per_sort_elem_cumu_max_left, per_sort_elem_cumu_max_right. *)
+(*   intros * HRR'. *)
+(*   split; intros []; econstructor; try eassumption; *)
+(*     apply HRR'; eassumption. *)
 (* Qed. *)
 
-(* Lemma per_ctx_subtyp_refl1 : forall Γ Δ R, *)
-(*     {{ EF Γ ≈ Δ ∈ per_ctx_env ↘ R }} -> *)
-(*     {{ SubE Γ <: Δ }}. *)
-(* Proof. *)
-(*   induction 1; mauto. *)
-
-(*   assert (exists R, {{ EF Γ , A ≈ Γ' , A' ∈ per_ctx_env ↘ R }}) by *)
-(*     (eexists; eapply per_ctx_env_cons'; eassumption). *)
-(*   destruct_all. *)
-(*   econstructor; try solve [saturate_refl; mauto 2]. *)
-(*   intros. *)
-(*   destruct_rel_typ. *)
-(*   simplify_evals. *)
-(*   eauto using per_subtyp_refl1. *)
+(* Lemma per_bot_sym {P : PtsSig} : forall m n : domain_ne P, *)
+(*     {{ Dom m ≈ n ∈ per_bot }} -> *)
+(*     {{ Dom n ≈ m ∈ per_bot }}. *)
+(* Proof with solve [eauto]. *)
+(*   intros * H s. *)
+(*   pose proof H s. *)
+(*   destruct_conjs... *)
 (* Qed. *)
 
-(* Lemma per_ctx_subtyp_refl2 : forall Γ Δ R, *)
-(*     {{ EF Γ ≈ Δ ∈ per_ctx_env ↘ R }} -> *)
-(*     {{ SubE Δ <: Γ }}. *)
-(* Proof. *)
-(*   intros. symmetry in H. eauto using per_ctx_subtyp_refl1. *)
+(* #[export] *)
+(* Hint Resolve per_bot_sym : mcpts. *)
+
+(* Lemma per_bot_trans {P : PtsSig} : forall m n l : domain_ne P, *)
+(*     {{ Dom m ≈ n ∈ per_bot }} -> *)
+(*     {{ Dom n ≈ l ∈ per_bot }} -> *)
+(*     {{ Dom m ≈ l ∈ per_bot }}. *)
+(* Proof with solve [eauto]. *)
+(*   intros * Hmn Hnl s. *)
+(*   pose proof (Hmn s, Hnl s). *)
+(*   destruct_conjs. *)
+(*   functional_read_rewrite_clear... *)
 (* Qed. *)
 
-(* Lemma per_ctx_subtyp_trans : forall Γ1 Γ2, *)
-(*     {{ SubE Γ1 <: Γ2 }} -> *)
-(*     forall Γ3, *)
-(*       {{ SubE Γ2 <: Γ3 }} -> *)
-(*       {{ SubE Γ1 <: Γ3 }}. *)
-(* Proof. *)
-(*   induction 1; intros; *)
-(*     dir_inversion_by_head per_ctx_subtyp; subst; *)
-(*     repeat invert_per_ctx_envs; *)
-(*     mauto 1; clear_PER. *)
+(* #[export] *)
+(* Hint Resolve per_bot_trans : mcpts. *)
 
-(*   handle_per_ctx_env_irrel. *)
-(*   econstructor; try eassumption. *)
-(*   - firstorder. *)
-(*   - instantiate (1 := max i i0). *)
-(*     intros. *)
-(*     assert {{ Dom ρ ≈ ρ' ∈ tail_rel0 }} *)
-(*       by (apply_relation_equivalence; eapply per_ctx_env_subtyping; revgoals; eassumption). *)
-(*     saturate_refl_for tail_rel. *)
-(*     destruct_rel_typ. *)
+(* #[export] *)
+(* Instance per_bot_PER {P : PtsSig} : PER (@per_bot P). *)
+(* Proof. *)
+(*   split. *)
+(*   - eauto using per_bot_sym. *)
+(*   - eauto using per_bot_trans. *)
+(* Qed. *)
+
+(* Lemma var_per_bot {P : PtsSig} : forall {n}, *)
+(*     {{ Dom !n ≈ !n ∈ @per_bot P }}. *)
+(* Proof. *)
+(*   intros ? ?. repeat econstructor. *)
+(* Qed. *)
+
+(* #[export] *)
+(* Hint Resolve var_per_bot : mcpts. *)
+
+(* Lemma per_top_sym {P : PtsSig} : forall m n : domain_nf P, *)
+(*     {{ Dom m ≈ n ∈ per_top }} -> *)
+(*     {{ Dom n ≈ m ∈ per_top }}. *)
+(* Proof with solve [eauto]. *)
+(*   intros * H s. *)
+(*   pose proof H s. *)
+(*   destruct_conjs... *)
+(* Qed. *)
+
+(* #[export] *)
+(* Hint Resolve per_top_sym : mcpts. *)
+
+(* Lemma per_top_trans {P : PtsSig} : forall m n l : domain_nf P, *)
+(*     {{ Dom m ≈ n ∈ per_top }} -> *)
+(*     {{ Dom n ≈ l ∈ per_top }} -> *)
+(*     {{ Dom m ≈ l ∈ per_top }}. *)
+(* Proof with solve [eauto]. *)
+(*   intros * Hmn Hnl s. *)
+(*   pose proof (Hmn s, Hnl s). *)
+(*   destruct_conjs. *)
+(*   functional_read_rewrite_clear... *)
+(* Qed. *)
+
+(* #[export] *)
+(* Hint Resolve per_top_trans : mcpts. *)
+
+(* #[export] *)
+(* Instance per_top_PER {P : PtsSig} : PER (@per_top P). *)
+(* Proof. *)
+(*   split. *)
+(*   - eauto using per_top_sym. *)
+(*   - eauto using per_top_trans. *)
+(* Qed. *)
+
+(* Lemma per_bot_then_per_top {P : PtsSig} : forall (m : domain_ne P) m' a a' b b' c c', *)
+(*     {{ Dom m ≈ m' ∈ per_bot }} -> *)
+(*     {{ Dom ⇓ (⇑ a b) ⇑ c m ≈ ⇓ (⇑ a' b') ⇑ c' m' ∈ per_top }}. *)
+(* Proof. *)
+(*   intros * H s. *)
+(*   pose proof H s. *)
+(*   destruct_conjs. *)
+(*   eexists; split; constructor; eassumption. *)
+(* Qed. *)
+
+(* #[export] *)
+(* Hint Resolve per_bot_then_per_top : mcpts. *)
+
+(* Lemma per_top_typ_sym {P : PtsSig} : forall m n : domain P, *)
+(*     {{ Dom m ≈ n ∈ per_top_typ }} -> *)
+(*     {{ Dom n ≈ m ∈ per_top_typ }}. *)
+(* Proof with solve [eauto]. *)
+(*   intros * H s. *)
+(*   pose proof H s. *)
+(*   destruct_conjs... *)
+(* Qed. *)
+
+(* #[export] *)
+(* Hint Resolve per_top_typ_sym : mcpts. *)
+
+(* Lemma per_top_typ_trans {P : PtsSig} : forall m n l : domain P, *)
+(*     {{ Dom m ≈ n ∈ per_top_typ }} -> *)
+(*     {{ Dom n ≈ l ∈ per_top_typ }} -> *)
+(*     {{ Dom m ≈ l ∈ per_top_typ }}. *)
+(* Proof with solve [eauto]. *)
+(*   intros * Hmn Hnl s. *)
+(*   pose proof (Hmn s, Hnl s). *)
+(*   destruct_conjs. *)
+(*   functional_read_rewrite_clear... *)
+(* Qed. *)
+
+(* #[export] *)
+(* Hint Resolve per_top_typ_trans : mcpts. *)
+
+(* #[export] *)
+(* Instance per_top_typ_PER {P : PtsSig} : PER (@per_top_typ P). *)
+(* Proof. *)
+(*   split. *)
+(*   - eauto using per_top_typ_sym. *)
+(*   - eauto using per_top_typ_trans. *)
+(* Qed. *)
+
+
+(* Lemma per_ne_sym {P : PtsSig} : forall m n : domain P, *)
+(*     {{ Dom m ≈ n ∈ per_ne }} -> *)
+(*     {{ Dom n ≈ m ∈ per_ne }}. *)
+(* Proof with mautosolve. *)
+(*   intros * []. *)
+(*   econstructor... *)
+(* Qed. *)
+
+(* #[export] *)
+(* Hint Resolve per_ne_sym : mcpts. *)
+
+(* Lemma per_ne_trans {P : PtsSig} : forall m n l : domain P, *)
+(*     {{ Dom m ≈ n ∈ per_ne }} -> *)
+(*     {{ Dom n ≈ l ∈ per_ne }} -> *)
+(*     {{ Dom m ≈ l ∈ per_ne }}. *)
+(* Proof with mautosolve. *)
+(*   intros * []. *)
+(*   inversion_clear 1. *)
+(*   econstructor... *)
+(* Qed. *)
+
+(* #[export] *)
+(* Hint Resolve per_ne_trans : mcpts. *)
+
+(* #[export] *)
+(* Instance per_ne_PER {P : PtsSig} : PER (@per_ne P). *)
+(* Proof. *)
+(*   split. *)
+(*   - eauto using per_ne_sym. *)
+(*   - eauto using per_ne_trans. *)
+(* Qed. *)
+
+(* Add Parametric Morphism {P : PtsSig} {pred_P : PredicativeSig P} s (per_sort_rec : forall s', pred_rel P pred_P s' s -> relation (domain P)) : (per_sort_elem_core P pred_P s per_sort_rec) *)
+(*     with signature (@relation_equivalence (domain P)) ==> eq ==> eq ==> iff as per_sort_elem_core_morphism_iff. *)
+(* Proof with mautosolve. *)
+(*   simpl. *)
+(*   intros R R' HRR'. *)
+
+(*   split; intros Horig; [gen R' | gen R]; *)
+(*     induction Horig; *)
+(*     eauto; *)
+(*     try (etransitivity; [symmetry + idtac|]; eassumption); *)
+(*     intros; *)
+(*     destruct_rel_mod_eval; *)
+(*     econstructor; mauto 3. *)
+(*   1-3: rewrite <- HRR'; mauto. *)
+(*   all: rewrite HRR'; mauto. *)
+(* Qed. *)
+
+(* Add Parametric Morphism {P : PtsSig} {pred_P : PredicativeSig P} s : (per_sort_elem P pred_P s) *)
+(*     with signature (@relation_equivalence (domain P)) ==> eq ==> eq ==> iff as per_sort_elem_morphism_iff. *)
+(* Proof with mautosolve. *)
+(*   simp per_sort_elem. *)
+(*   intros R R' HRR'. *)
+
+(*   split; intros Horig; [gen R' | gen R]; *)
+  
+(*     induction Horig; *)
+(*     eauto; *)
+(*     try (etransitivity; [symmetry + idtac|]; eassumption); *)
+(*     intros; *)
+(*     destruct_rel_mod_eval; *)
+(*     econstructor; mauto 3. *)
+(*   1-3: rewrite <- HRR'; mauto. *)
+(*   all: rewrite HRR'; mauto. *)
+(* Qed. *)
+
+
+(* Add Parametric Morphism {P : PtsSig} {pred_P : PredicativeSig P} s per_sort_rec : (per_sort_elem_core P pred_P s per_sort_rec) *)
+(*     with signature (@relation_equivalence (domain P)) ==> (@relation_equivalence (domain P)) as per_sort_elem_core_morphism_relation_equivalence. *)
+(* Proof with mautosolve. *)
+(*   intros * H ? ?. *)
+(*   simpl. *)
+(*   rewrite H. *)
+(*   reflexivity. *)
+(* Qed. *)
+
+(* Add Parametric Morphism {P : PtsSig} {pred_P : PredicativeSig P} s : (per_sort_elem P pred_P s) *)
+(*     with signature (@relation_equivalence (domain P)) ==> (@relation_equivalence (domain P)) as per_sort_elem_morphism_relation_equivalence. *)
+(* Proof with mautosolve. *)
+(*   intros * H ? ?. *)
+(*   simpl. *)
+(*   rewrite H. *)
+(*   reflexivity. *)
+(* Qed. *)
+
+(* Add Parametric Morphism {P : PtsSig} {pred_P : PredicativeSig P} s per_sort_rec A ρ A' ρ' : (rel_typ pred_P s per_sort_rec A ρ A' ρ') *)
+(*     with signature (@relation_equivalence (domain P)) ==> iff as rel_typ_morphism. *)
+(* Proof. *)
+(*   intros * HRR'. *)
+(*   split; intros []; econstructor; try eassumption; *)
+(*     [setoid_rewrite <- HRR' | setoid_rewrite HRR']; eassumption. *)
+(* Qed. *)
+
+(* Lemma domain_app_per {P : PtsSig} : forall (f : domain_ne P) f' a a', *)
+(*   {{ Dom f ≈ f' ∈ per_bot }} -> *)
+(*   {{ Dom a ≈ a' ∈ per_top }} -> *)
+(*   {{ Dom f a ≈ f' a' ∈ per_bot }}. *)
+(* Proof. *)
+(*   intros. intros s. *)
+(*   destruct (H s) as [? []]. *)
+(*   destruct (H0 s) as [? []]. *)
+(*   mauto. *)
+(* Qed. *)
+
+(* Ltac rewrite_relation_equivalence_left := *)
+(*   repeat match goal with *)
+(*     | H : ?R1 <~> ?R2 |- _ => *)
+(*         try setoid_rewrite H; *)
+(*         (on_all_hyp: fun H' => assert_fails (unify H H'); unmark H; setoid_rewrite H in H'); *)
+(*         let T := type of H in *)
+(*         fold (id T) in H *)
+(*     end; unfold id in *. *)
+
+(* Ltac rewrite_relation_equivalence_right := *)
+(*   repeat match goal with *)
+(*     | H : ?R1 <~> ?R2 |- _ => *)
+(*         try setoid_rewrite <- H; *)
+(*         (on_all_hyp: fun H' => assert_fails (unify H H'); unmark H; setoid_rewrite <- H in H'); *)
+(*         let T := type of H in *)
+(*         fold (id T) in H *)
+(*     end; unfold id in *. *)
+
+(* Ltac clear_relation_equivalence := *)
+(*   repeat match goal with *)
+(*     | H : ?R1 <~> ?R2 |- _ => *)
+(*         (unify R1 R2; clear H) + (is_var R1; clear R1 H) + (is_var R2; clear R2 H) *)
+(*     end. *)
+
+(* Ltac apply_relation_equivalence := *)
+(*   clear_relation_equivalence; *)
+(*   rewrite_relation_equivalence_right; *)
+(*   clear_relation_equivalence; *)
+(*   rewrite_relation_equivalence_left; *)
+(*   clear_relation_equivalence. *)
+
+(* Lemma per_sort_elem_right_irrel {P : PtsSig} {pred_P : PredicativeSig P} : forall s per_sort_rec R a b R' b', *)
+(*     {{ DF a ≈ b ∈ per_sort_elem_core P pred_P s per_sort_rec ↘ R }} -> *)
+(*     {{ DF a ≈ b' ∈ per_sort_elem_core P pred_P s per_sort_rec ↘ R' }} -> *)
+(*     (R <~> R'). *)
+(* Proof with (destruct_rel_mod_eval; destruct_rel_mod_app; functional_eval_rewrite_clear; econstructor; intuition). *)
+(*   simpl. *)
+(*   intros * Horig. *)
+(*   remember a as a' in |- *. *)
+(*   gen a' b' R'. *)
+
+(*   induction Horig ; eapply (per_sort_elem_core_strong_ind P pred_P); mauto.     *)
+(*   - intros. *)
+(*     subst. *)
+(*     dependent destruction H4. *)
+(*     assert (proj1 (ord_ax P pred_P s0 s_elem ax_s1_s_elem) = proj1 (ord_ax P pred_P s0 s_elem ax_s1_s_elem1)) by (eapply (pred_irrel P pred_P s0 s_elem); mauto).     *)
+(*     rewrite <- H in *. *)
+(*     apply_relation_equivalence. *)
+(*     reflexivity. *)
+(*   - intros. *)
+(*     subst. *)
+(*     dependent destruction H3. *)
+(*     assert (proj1 (ord_ax P pred_P s0 s_elem ax_s1_s_elem) = proj1 (ord_ax P pred_P s0 s_elem ax_s1_s_elem0)) by (eapply (pred_irrel P pred_P s0 s_elem); mauto).     *)
+(*     rewrite <- H in *. *)
+(*     apply_relation_equivalence. *)
+(*     reflexivity. *)
+(*   - intros * HMono * Heq HE IH * Heq' Hright. *)
+(*     subst. *)
+(*     dependent destruction Hright; *)
+(*       apply_relation_equivalence. *)
+(*     split; intros. *)
+(*     + admit. *)
+(*     +  *)
+    
+(*     admit. *)
+(*   - intros. *)
+(*     subst. *)
+(*     dependent destruction H4. *)
+(*     apply_relation_equivalence. *)
+(*     admit. *)
+(*   - intros; subst. *)
+(*     dependent destruction H3. *)
+(*     apply_relation_equivalence. *)
+(*     reflexivity. *)
+   
+(*   (* induction Horig. *) *)
+(*   (* - intros. *) *)
+(*   (*   subst. *) *)
+(*   (*   inversion H1. *) *)
+(*   (*   subst.     *) *)
+    
+(*   (*   assert (proj1 (ord_ax P pred_P s0 s_elem ax_s1_s_elem) = proj1 (ord_ax P pred_P s0 s_elem ax_s1_s_elem0)) by (eapply (pred_irrel P pred_P s0 s_elem); mauto). *) *)
+(*   (*   rewrite <- H in *. *) *)
+(*   (*   apply_relation_equivalence. *) *)
+(*   (*   reflexivity. *) *)
+
+(*   (* - intros * Heq Hright. *) *)
+(*   (*   subst.     *) *)
+(*   (*   dependent destruction Hright; *) *)
+(*   (*     apply_relation_equivalence. *) *)
+(*   (*   split; intros. *) *)
+(*   (*   + admit. *) *)
+(*   (*   + admit. *) *)
+(*   (* - intros.     *) *)
+(*   (*   subst. *) *)
+(*   (*   dependent destruction H1. *) *)
+(*   (*   apply_relation_equivalence. *) *)
+(*   (*   reflexivity. *) *)
+      
+(* Admitted. *)
+
+(* #[local] *)
+(* Ltac per_sort_elem_right_irrel_assert1 := *)
+(*   match goal with *)
+(*   | H1 : {{ DF ^?a ≈ ^?b ∈ per_sort_elem_core ?s ?psr ↘ ?R1 }}, *)
+(*       H2 : {{ DF ^?a ≈ ^?b' ∈ per_sort_elem ?s ?psr ↘ ?R2 }} |- _ => *)
+(*       assert_fails (unify R1 R2); *)
+(*       match goal with *)
+(*       | H : R1 <~> R2 |- _ => fail 1 *)
+(*       | H : R2 <~> R1 |- _ => fail 1 *)
+(*       | _ => assert (R1 <~> R2) by (eapply per_sort_elem_right_irrel; [apply H1 | apply H2]) *)
+(*       end *)
+(*   end. *)
+(* #[local] *)
+(* Ltac per_sort_elem_right_irrel_assert := repeat per_sort_elem_right_irrel_assert1. *)
+
+
+(* Lemma per_sort_elem_sym {P : PtsSig} {pred_P : PredicativeSig P} : forall s per_sort_rec R a b, *)
+(*     {{ DF a ≈ b ∈ per_sort_elem_core P pred_P s per_sort_rec ↘ R }} -> *)
+(*     {{ DF b ≈ a ∈ per_sort_elem_core P pred_P s per_sort_rec ↘ R }} /\ *)
+(*       (forall m m', *)
+(*           {{ Dom m ≈ m' ∈ R }} -> *)
+(*           {{ Dom m' ≈ m ∈ R }}). *)
+(* Proof with mautosolve. *)
+(*   (* simpl. *) *)
+(*   (* intros s per_sort_rec R a b Horig.    *) *)
+    
+(*   (* apply per_sort_elem_core_strong_ind with (s:=s) (motive:=fun s per_sort_rec R a b => per_sort_elem_core P pred_P s per_sort_rec R b a /\ (forall m m' : domain P, R m m' -> R m' m)); intros; subst. *) *)
+(*   (* - split. *) *)
+(*   (*   +  *) *)
+(*   (*     apply per_sort_elem_core_sort with (ax_s1_s_elem := ax_s1_s_elem). exact per_sort_rec_s1.  auto.  auto. *) *)
+(*   (*   + intros.       *) *)
+(*   (*     rewrite H0 in *. *) *)
+(*   (*     eapply H1 with (A := m) (B := m'); mauto 2. *) *)
+      
+
+      
+(*   (*     eapply proj1. *) *)
+(*   (*     eapply H1; mauto 2. *) *)
+      
+      
+(*   (* induction 1 using per_sort_elem_core_strong_ind; subst. *) *)
+(*   (* - split. *) *)
+(*   (*   + apply per_sort_elem_core_sort'; firstorder. *) *)
+(*   (*   + intros. *) *)
+(*   (*     rewrite H1 in *. *) *)
+(*   (*     destruct_by_head (@per_sort P). *) *)
+(*   (*     eexists. *) *)
+(*   (*     eapply proj1... *) *)
+
+(*   (* - destruct_conjs. *) *)
+(*   (*   split. *) *)
+(*   (*   + basic_per_sort_elem_econstructor; eauto. *) *)
+(*   (*     * admit. *) *)
+(*   (*     * intros. *) *)
+(*   (*     assert (in_rel n' n) by eauto. *) *)
+(*   (*     assert (in_rel n n) by (etransitivity; eassumption). *) *)
+(*   (*     destruct_all. *) *)
+(*   (*     destruct_rel_mod_eval. *) *)
+(*   (*     functional_eval_rewrite_clear. *) *)
+(*   (*     econstructor; eauto. *) *)
+(*   (*     per_sort_elem_right_irrel_assert. *) *)
+(*   (*     apply_relation_equivalence. *) *)
+(*   (*     (* eassumption *) *) *)
+(*   (*     admit. *) *)
+(*   (*   + apply_relation_equivalence. *) *)
+(*   (*     intros. *) *)
+(*   (*     assert (in_rel n' n) by eauto. *) *)
+(*   (*     assert (in_rel n n) by (etransitivity; eassumption). *) *)
+(*   (*     destruct_rel_mod_eval. *) *)
+(*   (*     destruct_rel_mod_app. *) *)
+(*   (*     functional_eval_rewrite_clear. *) *)
+(*   (*     econstructor; eauto. *) *)
+(*   (*     per_sort_elem_right_irrel_assert. *) *)
+(*   (*     (* intuition. *) *) *)
+(*   (*     admit. *) *)
+      
+(*   (* - split; [basic_per_sort_elem_econstructor | apply_relation_equivalence]; mauto 3. *) *)
+(* Admitted. *)
+
+
+(* Corollary per_sort_sym {P : PtsSig} {pred_P : PredicativeSig P} : forall s per_sort_rec R a b, *)
+(*     {{ DF a ≈ b ∈ per_sort_elem_core P pred_P s per_sort_rec ↘ R }} -> *)
+(*     {{ DF b ≈ a ∈ per_sort_elem_core P pred_P s per_sort_rec ↘ R }}. *)
+(* Proof.   *)
+(*   intros * ?%per_sort_elem_sym. *)
+(*   firstorder. *)
+(* Qed. *)
+
+(* Corollary per_sort_sym' {P : PtsSig} {pred_P : PredicativeSig P} : forall s a b, *)
+(*     {{ Dom a ≈ b ∈ per_sort pred_P s }} -> *)
+(*     {{ Dom b ≈ a ∈ per_sort pred_P s }}. *)
+(* Proof. *)
+(*   intros * [? ?%per_sort_elem_sym]. *)
+(*   firstorder. *)
+(* Qed. *)
+
+(* Corollary per_elem_sym {P : PtsSig} {pred_P : PredicativeSig P} : forall s R a b m m', *)
+(*     {{ DF a ≈ b ∈ per_sort_elem P pred_P s ↘ R }} -> *)
+(*     {{ Dom m ≈ m' ∈ R }} -> *)
+(*     {{ Dom m' ≈ m ∈ R }}. *)
+(* Proof. *)
+(*   intros * ?%per_sort_elem_sym. *)
+(*   firstorder. *)
+(* Qed. *)
+
+(* Corollary per_sort_elem_left_irrel {P : PtsSig} {pred_P : PredicativeSig P} : forall s s' R a b R' a', *)
+(*     {{ DF a ≈ b ∈ per_sort_elem P pred_P s ↘ R }} -> *)
+(*     {{ DF a' ≈ b ∈ per_sort_elem P pred_P s' ↘ R' }} -> *)
+(*     (R <~> R'). *)
+(* Proof. *)
+(*   intros * ?%per_sort_sym ?%per_sort_sym. *)
+(*   eauto using per_sort_elem_right_irrel. *)
+(* Qed. *)
+
+(* Corollary per_sort_elem_cross_irrel {P : PtsSig} {pred_P : PredicativeSig P} : forall s s' R a b R' b', *)
+(*     {{ DF a ≈ b ∈ per_sort_elem P pred_P s ↘ R }} -> *)
+(*     {{ DF b' ≈ a ∈ per_sort_elem P pred_P s' ↘ R' }} -> *)
+(*     (R <~> R'). *)
+(* Proof. *)
+(*   intros * ? ?%per_sort_sym. *)
+(*   eauto using per_sort_elem_right_irrel. *)
+(* Qed. *)
+
+(* Ltac do_per_sort_elem_irrel_assert1 := *)
+(*   let tactic_error o1 o2 := fail 2 "per_sort_elem_irrel biconditional between" o1 "and" o2 "cannot be solved" in *)
+(*   match goal with *)
+(*   | H1 : {{ DF ^?a ≈ ^_ ∈ per_sort_elem ?P ?pred_P ?s ↘ ?R1 }}, *)
+(*       H2 : {{ DF ^?a ≈ ^_ ∈ per_sort_elem ?P ?pred_P ?s' ↘ ?R2 }} |- _ => *)
+(*       assert_fails (unify R1 R2); *)
+(*       match goal with *)
+(*       | H : R1 <~> R2 |- _ => fail 1 *)
+(*       | H : R2 <~> R1 |- _ => fail 1 *)
+(*       | _ => assert (R1 <~> R2) by (eapply per_sort_elem_right_irrel; [apply H1 | apply H2]) || tactic_error R1 R2 *)
+(*       end *)
+(*   | H1 : {{ DF ^_ ≈ ^?b ∈ per_sort_elem ?P ?pred_P ?s ↘ ?R1 }}, *)
+(*       H2 : {{ DF ^_ ≈ ^?b ∈ per_sort_elem ?P ?pred_P ?s' ↘ ?R2 }} |- _ => *)
+(*       assert_fails (unify R1 R2); *)
+(*       match goal with *)
+(*       | H : R1 <~> R2 |- _ => fail 1 *)
+(*       | H : R2 <~> R1 |- _ => fail 1 *)
+(*       | _ => assert (R1 <~> R2) by (eapply per_sort_elem_left_irrel; [apply H1 | apply H2]) || tactic_error R1 R2 *)
+(*       end *)
+(*   | H1 : {{ DF ^?a ≈ ^_ ∈ per_sort_elem ?P ?pred_P ?s ↘ ?R1 }}, *)
+(*       H2 : {{ DF ^_ ≈ ^?a ∈ per_sort_elem ?P ?pred_P ?s' ↘ ?R2 }} |- _ => *)
+(*       (** Order matters less here as H1 and H2 cannot be exchanged *) *)
+(*       assert_fails (unify R1 R2); *)
+(*       match goal with *)
+(*       | H : R1 <~> R2 |- _ => fail 1 *)
+(*       | H : R2 <~> R1 |- _ => fail 1 *)
+(*       | _ => assert (R1 <~> R2) by (eapply per_sort_elem_cross_irrel; [apply H1 | apply H2]) || tactic_error R1 R2 *)
+(*       end *)
+(*   end. *)
+
+(* Ltac do_per_sort_elem_irrel_assert := *)
+(*   repeat do_per_sort_elem_irrel_assert1. *)
+
+(* Ltac handle_per_sort_elem_irrel := *)
+(*   functional_eval_rewrite_clear; *)
+(*   do_per_sort_elem_irrel_assert; *)
+(*   apply_relation_equivalence; *)
+(*   clear_dups. *)
+
+(* Lemma per_sort_elem_trans {P : PtsSig} {pred_P : PredicativeSig P} : forall s R a1 a2, *)
+(*     per_sort_elem P pred_P s R a1 a2 -> *)
+(*     (forall s' a3, *)
+(*         per_sort_elem P pred_P s' R a2 a3 -> *)
+(*         per_sort_elem P pred_P s R a1 a3) /\ *)
+(*       (forall m1 m2 m3, *)
+(*           R m1 m2 -> *)
+(*           R m2 m3 -> *)
+(*           R m1 m3). *)
+(* Proof with (basic_per_sort_elem_econstructor; mautosolve 4). *)
+(*   induction 1 using per_sort_elem_ind; *)
+(*     [> split; *)
+(*      [ intros * HT2; basic_invert_per_sort_elem HT2 *)
+(*      | intros * HTR1 HTR2; apply_relation_equivalence ] ..]; mauto. *)
+(*   - subst. mauto. *)
+(*   - (* sort case *) *)
+(*     subst. *)
+(*     destruct HTR1, HTR2. *)
+(*     functional_eval_rewrite_clear. *)
 (*     handle_per_sort_elem_irrel. *)
-(*     etransitivity; intuition mauto using per_subtyp_cumu_left, per_subtyp_cumu_right. *)
-(*   - econstructor; intuition. *)
-(*     + typeclasses eauto. *)
-(*     + solve_refl. *)
-(*   - econstructor; mauto 3. *)
-(*     + typeclasses eauto. *)
-(*     + solve_refl. *)
-(* Qed. *)
+(*     eexists. *)
+(*     specialize (H2 _ _ _ H0) as []. *)
+(*     intuition. *)
+(*   - (* pi case *) *)
+(*     destruct_conjs. *)
+(*     basic_per_sort_elem_econstructor; eauto. *)
+(*     + handle_per_sort_elem_irrel. *)
+(*       intuition. *)
+(*       admit. *)
+(*     + intros. *)
+(*       handle_per_sort_elem_irrel. *)
+(*       assert (in_rel n n') by (firstorder; admit). *)
+(*       assert (in_rel n n) by intuition. *)
+(*       assert (in_rel0 n n) by (intuition; admit). *)
+(*       destruct_rel_mod_eval. *)
+(*       functional_eval_rewrite_clear. *)
+(*       (* handle_per_sort_elem_irrel... *) *)
+(*       admit. *)
+(*   - (* fun case *) *)
+(*     intros. *)
+(*     assert (in_rel n n) by intuition. *)
+(*     destruct_rel_mod_eval. *)
+(*     destruct_rel_mod_app. *)
+(*     handle_per_sort_elem_irrel. *)
+(*     econstructor; eauto. *)
+(*     intuition. *)
+(*   - (* neut case *) *)
+(*     idtac... *)
+(* Admitted. *)
 
-(* #[export] *)
-(* Hint Resolve per_ctx_subtyp_trans : mcpts. *)
-
-(* #[export] *)
-(* Instance per_ctx_subtyp_trans_ins : Transitive per_ctx_subtyp. *)
+(* Corollary per_sort_trans {P : PtsSig} {pred_P : PredicativeSig P} : forall s s' R a1 a2 a3, *)
+(*     per_sort_elem P pred_P s R a1 a2 -> *)
+(*     per_sort_elem P pred_P s' R a2 a3 -> *)
+(*     per_sort_elem P pred_P s R a1 a3. *)
 (* Proof. *)
-(*   eauto using per_ctx_subtyp_trans. *)
+(*   intros * ?%per_sort_elem_trans. *)
+(*   firstorder. *)
 (* Qed. *)
+
+(* Corollary per_sort_trans' {P : PtsSig} {pred_P : PredicativeSig P} : forall s s' a1 a2 a3, *)
+(*     {{ Dom a1 ≈ a2 ∈ per_sort pred_P s }} -> *)
+(*     {{ Dom a2 ≈ a3 ∈ per_sort pred_P s' }} -> *)
+(*     {{ Dom a1 ≈ a3 ∈ per_sort pred_P s }}. *)
+(* Proof. *)
+(*   intros * [? ?] [? ?]. *)
+(*   handle_per_sort_elem_irrel. *)
+(*   firstorder mauto using per_sort_trans. *)
+(* Qed. *)
+
+(* Corollary per_elem_trans {P : PtsSig} {pred_P : PredicativeSig P} : forall s R a1 a2 m1 m2 m3, *)
+(*     per_sort_elem P pred_P s R a1 a2 -> *)
+(*     R m1 m2 -> *)
+(*     R m2 m3 -> *)
+(*     R m1 m3. *)
+(* Proof. *)
+(*   intros * ?% per_sort_elem_trans. *)
+(*   firstorder. *)
+(* Qed. *)
+
+(* #[export] *)
+(* Instance per_sort_PER {P : PtsSig} {pred_P : PredicativeSig P} {s R} : PER (per_sort_elem P pred_P s R). *)
+(* Proof. *)
+(*   split. *)
+(*   - auto using per_sort_sym. *)
+(*   - eauto using per_sort_trans. *)
+(* Qed. *)
+
+(* #[export] *)
+(* Instance per_sort_PER' {P : PtsSig} {pred_P : PredicativeSig P} {s} : PER (per_sort pred_P s). *)
+(* Proof. *)
+(*   split. *)
+(*   - auto using per_sort_sym'. *)
+(*   - eauto using per_sort_trans'. *)
+(* Qed. *)
+
+(* #[export] *)
+(* Instance per_elem_PER {P : PtsSig} {pred_P : PredicativeSig P} {s R a b} `(H : per_sort_elem P pred_P s R a b) : PER R. *)
+(* Proof. *)
+(*   split. *)
+(*   - pose proof (fun m m' => per_elem_sym _ _ _ _ m m' H). eauto. *)
+(*   - pose proof (fun m0 m1 m2 => per_elem_trans _ _ _ _ m0 m1 m2 H); eauto. *)
+(* Qed. *)
+
+(* (** These lemmas get rid of the unnecessary PER premises. *) *)
+(* Lemma per_sort_elem_pi' {P : PtsSig} {pred_P : PredicativeSig P} : *)
+(*   forall s_in s_out s (r : Ru P s_in s_out s) a a' ρ B ρ' B' *)
+(*     (in_rel : relation (domain P)) *)
+(*     (out_rel : forall {c c'} (equiv_c_c' : {{ Dom c ≈ c' ∈ in_rel }}), relation (domain P)) *)
+(*     elem_rel, *)
+(*     {{ DF a ≈ a' ∈ per_sort_elem P pred_P s_in ↘ in_rel}} -> *)
+(*     (forall {c c'} (equiv_c_c' : {{ Dom c ≈ c' ∈ in_rel }}), *)
+(*         rel_mod_eval (per_sort_elem P pred_P s_out) B d{{{ ρ ↦ c }}} B' d{{{ ρ' ↦ c' }}} (out_rel equiv_c_c')) -> *)
+(*     (elem_rel <~> fun f f' => forall c c' (equiv_c_c' : {{ Dom c ≈ c' ∈ in_rel }}), rel_mod_app f c f' c' (out_rel equiv_c_c')) -> *)
+(*     {{ DF Π r a ρ B ≈ Π r a' ρ' B' ∈ per_sort_elem P pred_P s ↘ elem_rel }}. *)
+(* Proof. *)
+(*   intros. *)
+(*   basic_per_sort_elem_econstructor; eauto. *)
+(*   (* typeclasses eauto. *) *)
+(*   admit. *)
+(* Admitted. *)
+
+
+(* Ltac per_sort_elem_econstructor := *)
+(*   (repeat intro; hnf; (eapply per_sort_elem_pi')) + basic_per_sort_elem_econstructor. *)
+
+(* #[export] *)
+(* Hint Resolve per_sort_elem_pi' : mcpts. *)
+
+(* Lemma per_sort_elem_pi_clean_inversion {P : PtsSig} {pred_P : PredicativeSig P} : forall {s_in s_out s} {r : Ru P s_in s_out s} {a a' in_rel ρ ρ' B B' elem_rel}, *)
+(*     {{ DF a ≈ a' ∈ per_sort_elem P pred_P s_in ↘ in_rel }} -> *)
+(*     {{ DF Π r a ρ B ≈ Π r a' ρ' B' ∈ per_sort_elem P pred_P s ↘ elem_rel }} -> *)
+(*     exists (out_rel : forall {n n'} (equiv_n_n' : {{ Dom n ≈ n' ∈ in_rel }}), relation (domain P)), *)
+(*       (forall n n' (equiv_n_n' : {{ Dom n ≈ n' ∈ in_rel }}), *)
+(*           rel_mod_eval (per_sort_elem P pred_P s_out) B d{{{ ρ ↦ n }}} B' d{{{ ρ' ↦ n' }}} (out_rel equiv_n_n')) /\ *)
+(*         (elem_rel <~> fun f f' => forall n n' (equiv_n_n' : {{ Dom n ≈ n' ∈ in_rel }}), rel_mod_app f n f' n' (out_rel equiv_n_n')). *)
+(* Proof. *)
+(*   intros * Ha HΠ. *)
+(*   basic_invert_per_sort_elem HΠ. *)
+(*   handle_per_sort_elem_irrel. *)
+(*   eexists. *)
+(*   split. *)
+(*   - instantiate (1 := fun n n' (equiv_n_n' : in_rel n n') m m' => *)
+(*                         forall R, *)
+(*                           rel_typ pred_P s_out B d{{{ ρ ↦ n }}} B' d{{{ ρ' ↦ n' }}} R -> *)
+(*                           R m m'). *)
+(*     intros. *)
+(*     (* assert (in_rel0 n n') by intuition. *) *)
+(*     (* (on_all_hyp: destruct_rel_by_assumption in_rel0). *) *)
+(*     (* econstructor; eauto. *) *)
+(*     (* apply -> per_sort_elem_morphism_iff; eauto. *) *)
+(*     (* split; intuition. *) *)
+(*     (* destruct_by_head rel_typ. *) *)
+(*     (* handle_per_sort_elem_irrel. *) *)
+(*     (* intuition. *) *)
+(*     admit. *)
+(*   - (* split; intros; *) *)
+(*     (*   [assert (in_rel0 n n') by intuition; (on_all_hyp: destruct_rel_by_assumption in_rel0) *) *)
+(*     (*   | assert (in_rel n n') by intuition; (on_all_hyp: destruct_rel_by_assumption in_rel)]; *) *)
+(*     (*   econstructor; intuition. *) *)
+(*     (* destruct_by_head rel_typ. *) *)
+(*     (* handle_per_sort_elem_irrel. *) *)
+(*     (* intuition. *) *)
+(*     admit. *)
+(* Admitted. *)
+
+(* Ltac invert_per_sort_elem H := *)
+(*   (unshelve eapply (per_sort_elem_pi_clean_inversion _) in H; shelve_unifiable; [eassumption |]; destruct H as [? []]) *)
+(*   + basic_invert_per_sort_elem H. *)
+
+(* Ltac invert_per_sort_elems := match_by_head per_sort_elem ltac:(fun H => directed invert_per_sort_elem H). *)
+
+
+(* (* These are all lemmas about subtyping.  We might need to replace them with something else *) *)
+
+(* (* Lemma per_subtyp_to_sort_elem : forall a b i, *) *)
+(* (*     {{ Sub a <: b at i }} -> *) *)
+(* (*     exists R R', *) *)
+(* (*       {{ DF a ≈ a ∈ per_sort_elem i ↘ R }} /\ *) *)
+(* (*         {{ DF b ≈ b ∈ per_sort_elem i ↘ R' }}. *) *)
+(* (* Proof. *) *)
+(* (*   destruct 1; do 2 eexists; mauto; *) *)
+(* (*     split; *) *)
+(* (*     try (etransitivity; try eassumption; symmetry; eassumption); *) *)
+(* (*     per_sort_elem_econstructor; mauto 3; *) *)
+(* (*     try apply Equivalence_Reflexive. *) *)
+
+(* (*   lia. *) *)
+(* (* Qed. *) *)
+
+(* (* Lemma per_elem_subtyping : forall A B i, *) *)
+(* (*     {{ Sub A <: B at i }} -> *) *)
+(* (*     forall R R' a b, *) *)
+(* (*       {{ DF A ≈ A ∈ per_sort_elem i ↘ R }} -> *) *)
+(* (*       {{ DF B ≈ B ∈ per_sort_elem i ↘ R' }} -> *) *)
+(* (*       R a b -> *) *)
+(* (*       R' a b. *) *)
+(* (* Proof. *) *)
+(* (*   induction 1; intros; *) *)
+(* (*     handle_per_sort_elem_irrel; *) *)
+(* (*     saturate_refl; *) *)
+(* (*     invert_per_sort_elems; *) *)
+(* (*     handle_per_sort_elem_irrel; *) *)
+(* (*     clear_refl_eqs; *) *)
+(* (*     trivial. *) *)
+(* (*   - firstorder mauto. *) *)
+(* (*   - intros. *) *)
+(* (*     handle_per_sort_elem_irrel. *) *)
+(* (*     destruct_rel_mod_eval. *) *)
+(* (*     saturate_refl_for per_sort_elem. *) *)
+(* (*     destruct_rel_mod_app. *) *)
+(* (*     simplify_evals. *) *)
+(* (*     econstructor; eauto. *) *)
+(* (*     intuition. *) *)
+(* (* Qed. *) *)
+
+(* (* Lemma per_elem_subtyping_gen : forall a b i a' b' R R' m n, *) *)
+(* (*     {{ Sub a <: b at i }} -> *) *)
+(* (*     {{ DF a ≈ a' ∈ per_sort_elem i ↘ R }} -> *) *)
+(* (*     {{ DF b ≈ b' ∈ per_sort_elem i ↘ R' }} -> *) *)
+(* (*     R m n -> *) *)
+(* (*     R' m n. *) *)
+(* (* Proof. *) *)
+(* (*   intros. *) *)
+(* (*   eapply per_elem_subtyping; saturate_refl; try eassumption. *) *)
+(* (* Qed. *) *)
+
+(* (* Lemma per_subtyp_refl1 : forall a b i R, *) *)
+(* (*     {{ DF a ≈ b ∈ per_sort_elem i ↘ R }} -> *) *)
+(* (*     {{ Sub a <: b at i }}. *) *)
+(* (* Proof. *) *)
+(* (*   simpl; induction 1 using per_sort_elem_ind; *) *)
+(* (*     subst; *) *)
+(* (*     mauto; *) *)
+(* (*     destruct_all. *) *)
+(* (*     assert ({{ DF Π a ρ B ≈ Π a' ρ' B' ∈ per_sort_elem i ↘ elem_rel }}) *) *)
+(* (*       by (per_sort_elem_econstructor; intuition; destruct_rel_mod_eval; mauto). *) *)
+(* (*     saturate_refl_for per_sort_elem. *) *)
+(* (*     econstructor; eauto. *) *)
+(* (*     intros; *) *)
+(* (*       destruct_rel_mod_eval; *) *)
+(* (*       functional_eval_rewrite_clear; *) *)
+(* (*       trivial. *) *)
+(* (* Qed. *) *)
+
+(* (* #[export] *) *)
+(* (* Hint Resolve per_subtyp_refl1 : mcpts. *) *)
+
+(* (* Lemma per_subtyp_refl2 : forall a b i R, *) *)
+(* (*     {{ DF a ≈ b ∈ per_sort_elem i ↘ R }} -> *) *)
+(* (*     {{ Sub b <: a at i }}. *) *)
+(* (* Proof. *) *)
+(* (*   intros. *) *)
+(* (*   symmetry in H. *) *)
+(* (*   eauto using per_subtyp_refl1. *) *)
+(* (* Qed. *) *)
+
+(* (* #[export] *) *)
+(* (* Hint Resolve per_subtyp_refl2 : mcpts. *) *)
+
+(* (* Lemma per_subtyp_trans : forall a1 a2 i, *) *)
+(* (*     {{ Sub a1 <: a2 at i }} -> *) *)
+(* (*     forall a3, *) *)
+(* (*       {{ Sub a2 <: a3 at i }} -> *) *)
+(* (*       {{ Sub a1 <: a3 at i }}. *) *)
+(* (* Proof. *) *)
+(* (*   induction 1; intros ? Hsub; simpl in *. *) *)
+(* (*   1,2,5: progressive_inversion; mauto. *) *)
+(* (*   - econstructor; lia. *) *)
+(* (*   - dependent destruction Hsub. *) *)
+(* (*     handle_per_sort_elem_irrel. *) *)
+(* (*     econstructor; eauto. *) *)
+(* (*     + etransitivity; eassumption. *) *)
+(* (*     + intros. *) *)
+(* (*       invert_per_sort_elems. *) *)
+(* (*       handle_per_sort_elem_irrel. *) *)
+(* (*       saturate_refl_for in_rel1. *) *)
+(* (*       destruct_rel_mod_eval. *) *)
+(* (*       intuition. *) *)
+(* (*   - dependent destruction Hsub. *) *)
+(* (*     handle_per_sort_elem_irrel. *) *)
+(* (*     econstructor; etransitivity; eauto. *) *)
+(* (* Qed. *) *)
+
+(* (* #[export] *) *)
+(* (* Hint Resolve per_subtyp_trans : mcpts. *) *)
+
+(* (* #[export] *) *)
+(* (* Instance per_subtyp_trans_ins i : Transitive (per_subtyp i). *) *)
+(* (* Proof. *) *)
+(* (*   eauto using per_subtyp_trans. *) *)
+(* (* Qed. *) *)
+
+(* (* Lemma per_subtyp_transp : forall a b i a' b' R R', *) *)
+(* (*     {{ Sub a <: b at i }} -> *) *)
+(* (*     {{ DF a ≈ a' ∈ per_sort_elem i ↘ R }} -> *) *)
+(* (*     {{ DF b ≈ b' ∈ per_sort_elem i ↘ R' }} -> *) *)
+(* (*     {{ Sub a' <: b' at i }}. *) *)
+(* (* Proof. *) *)
+(* (*   mauto using per_subtyp_refl1, per_subtyp_refl2. *) *)
+(* (* Qed. *) *)
+
+(* (* Lemma per_subtyp_cumu : forall a1 a2 i, *) *)
+(* (*     {{ Sub a1 <: a2 at i }} -> *) *)
+(* (*     forall j, *) *)
+(* (*       i <= j -> *) *)
+(* (*       {{ Sub a1 <: a2 at j }}. *) *)
+(* (* Proof. *) *)
+(* (*   induction 1; intros; econstructor; mauto. *) *)
+(* (*   lia. *) *)
+(* (* Qed. *) *)
+
+(* (* #[export] *) *)
+(* (* Hint Resolve per_subtyp_cumu : mcpts. *) *)
+
+(* (* Lemma per_subtyp_cumu_left : forall a1 a2 i j, *) *)
+(* (*     {{ Sub a1 <: a2 at i }} -> *) *)
+(* (*     {{ Sub a1 <: a2 at max i j }}. *) *)
+(* (* Proof. *) *)
+(* (*   intros. eapply per_subtyp_cumu; try eassumption. *) *)
+(* (*   lia. *) *)
+(* (* Qed. *) *)
+
+(* (* Lemma per_subtyp_cumu_right : forall a1 a2 i j, *) *)
+(* (*     {{ Sub a1 <: a2 at i }} -> *) *)
+(* (*     {{ Sub a1 <: a2 at max j i }}. *) *)
+(* (* Proof. *) *)
+(* (*   intros. eapply per_subtyp_cumu; try eassumption. *) *)
+(* (*   lia. *) *)
+(* (* Qed. *) *)
+
+(* Add Parametric Morphism {P : PtsSig} {pred_P : PredicativeSig P} : (@per_ctx_env P pred_P) *)
+(*     with signature (@relation_equivalence (env P)) ==> eq ==> eq ==> iff as per_ctx_env_morphism_iff. *)
+(* Proof with mautosolve. *)
+(*   intros R R' HRR'. *)
+(*   split; intro Horig; [gen R' | gen R]; *)
+(*     induction Horig; econstructor; *)
+(*     apply_relation_equivalence; try reflexivity... *)
+(* Qed. *)
+
+(* Add Parametric Morphism {P : PtsSig} {pred_P : PredicativeSig P} : (@per_ctx_env P pred_P) *)
+(*     with signature (@relation_equivalence (env P)) ==> (@relation_equivalence (ctx P)) as per_ctx_env_morphism_relation_equivalence. *)
+(* Proof. *)
+(*   intros * HRR' Γ Γ'. *)
+(*   simpl. *)
+(*   rewrite HRR'. *)
+(*   reflexivity. *)
+(* Qed. *)
+
+(* Lemma per_ctx_env_right_irrel {P : PtsSig} {pred_P : PredicativeSig P} : forall Γ Δ Δ' R R', *)
+(*     {{ DF Γ ≈ Δ ∈ (@per_ctx_env P pred_P) ↘ R }} -> *)
+(*     {{ DF Γ ≈ Δ' ∈ (@per_ctx_env P pred_P) ↘ R' }} -> *)
+(*     R <~> R'. *)
+(* Proof with (destruct_rel_typ; handle_per_sort_elem_irrel; eexists; intuition). *)
+(*   intros * Horig; gen Δ' R'. *)
+(*   induction Horig; intros * Hright; *)
+(*     inversion Hright; subst; *)
+(*     apply_relation_equivalence; *)
+(*     try reflexivity. *)
+(*   specialize (IHHorig _ _ equiv_Γ_Γ'0). *)
+(*   intros ρ ρ'. *)
+(*   split; intros Hcons; dependent destruction Hcons. *)
+(*   - assert {{ Dom ρ ↯ ≈ ρ' ↯ ∈ tail_rel0 }} by intuition... *)
+(*     admit. *)
+(*   - assert {{ Dom ρ ↯ ≈ ρ' ↯ ∈ tail_rel }} by intuition... *)
+(*     admit. *)
+(* Admitted. *)
+
+(* Lemma per_ctx_env_sym {P : PtsSig} {pred_P : PredicativeSig P} : forall Γ Δ R, *)
+(*     {{ DF Γ ≈ Δ ∈ @per_ctx_env P pred_P ↘ R }} -> *)
+(*     {{ DF Δ ≈ Γ ∈ @per_ctx_env P pred_P ↘ R }} /\ *)
+(*       (forall ρ ρ', *)
+(*           {{ Dom ρ ≈ ρ' ∈ R }} -> *)
+(*           {{ Dom ρ' ≈ ρ ∈ R }}). *)
+(* Proof with solve [intuition]. *)
+(*   simpl. *)
+(*   (* induction 1; split; simpl in *; destruct_conjs; try econstructor; intuition; *) *)
+(*   (*   pose proof (@relation_equivalence_pointwise env). *) *)
+(*   (* - assert (tail_rel ρ' ρ) by eauto. *) *)
+(*   (*   assert (tail_rel ρ ρ) by (etransitivity; eassumption). *) *)
+(*   (*   destruct_rel_mod_eval. *) *)
+(*   (*   handle_per_sort_elem_irrel. *) *)
+(*   (*   econstructor; eauto. *) *)
+(*   (*   symmetry... *) *)
+(*   (* - apply_relation_equivalence. *) *)
+(*   (*   destruct_by_head cons_per_ctx_env. *) *)
+(*   (*   assert (tail_rel d{{{ ρ' ↯ }}} d{{{ ρ ↯ }}}) by eauto. *) *)
+(*   (*   assert (tail_rel d{{{ ρ ↯ }}} d{{{ ρ ↯ }}}) by (etransitivity; eassumption). *) *)
+(*   (*   destruct_rel_mod_eval. *) *)
+(*   (*   eexists; symmetry; handle_per_sort_elem_irrel; intuition. *) *)
+(* Admitted. *)
+
+(* Corollary per_ctx_sym {P : PtsSig} {pred_P : PredicativeSig P} : forall Γ Δ R, *)
+(*     {{ DF Γ ≈ Δ ∈ @per_ctx_env P pred_P ↘ R }} -> *)
+(*     {{ DF Δ ≈ Γ ∈ @per_ctx_env P pred_P ↘ R }}. *)
+(* Proof. *)
+(*   intros * ?%per_ctx_env_sym. *)
+(*   firstorder. *)
+(* Qed. *)
+
+(* Corollary per_env_sym {P : PtsSig} {pred_P : PredicativeSig P} : forall Γ Δ R ρ ρ', *)
+(*     {{ DF Γ ≈ Δ ∈ @per_ctx_env P pred_P ↘ R }} -> *)
+(*     {{ Dom ρ ≈ ρ' ∈ R }} -> *)
+(*     {{ Dom ρ' ≈ ρ ∈ R }}. *)
+(* Proof. *)
+(*   intros * ?%per_ctx_env_sym. *)
+(*   firstorder. *)
+(* Qed. *)
+
+(* Corollary per_ctx_env_left_irrel {P : PtsSig} {pred_P : PredicativeSig P} : forall Γ Γ' Δ R R', *)
+(*     {{ DF Γ ≈ Δ ∈ @per_ctx_env P pred_P ↘ R }} -> *)
+(*     {{ DF Γ' ≈ Δ ∈ @per_ctx_env P pred_P ↘ R' }} -> *)
+(*     R <~> R'. *)
+(* Proof. *)
+(*   intros * ?%per_ctx_sym ?%per_ctx_sym. *)
+(*   eauto using per_ctx_env_right_irrel. *)
+(* Qed. *)
+
+(* Corollary per_ctx_env_cross_irrel {P : PtsSig} {pred_P : PredicativeSig P} : forall Γ Δ Δ' R R', *)
+(*     {{ DF Γ ≈ Δ ∈ @per_ctx_env P pred_P ↘ R }} -> *)
+(*     {{ DF Δ' ≈ Γ ∈ @per_ctx_env P pred_P ↘ R' }} -> *)
+(*     R <~> R'. *)
+(* Proof. *)
+(*   intros * ? ?%per_ctx_sym. *)
+(*   eauto using per_ctx_env_right_irrel. *)
+(* Qed. *)
+
+(* Ltac do_per_ctx_env_irrel_assert1 := *)
+(*   let tactic_error o1 o2 := fail 3 "per_ctx_env_irrel equality between" o1 "and" o2 "cannot be solved" in *)
+(*   match goal with *)
+(*     | H1 : {{ DF ^?Γ ≈ ^_ ∈ per_ctx_env ↘ ?R1 }}, *)
+(*         H2 : {{ DF ^?Γ ≈ ^_ ∈ per_ctx_env ↘ ?R2 }} |- _ => *)
+(*         assert_fails (unify R1 R2); *)
+(*         match goal with *)
+(*         | H : R1 <~> R2 |- _ => fail 1 *)
+(*         | H : R2 <~> R1 |- _ => fail 1 *)
+(*         | _ => assert (R1 <~> R2) by (eapply per_ctx_env_right_irrel; [apply H1 | apply H2]) || tactic_error R1 R2 *)
+(*         end *)
+(*     | H1 : {{ DF ^_ ≈ ^?Δ ∈ per_ctx_env ↘ ?R1 }}, *)
+(*         H2 : {{ DF ^_ ≈ ^?Δ ∈ per_ctx_env ↘ ?R2 }} |- _ => *)
+(*         assert_fails (unify R1 R2); *)
+(*         match goal with *)
+(*         | H : R1 <~> R2 |- _ => fail 1 *)
+(*         | H : R2 <~> R1 |- _ => fail 1 *)
+(*         | _ => assert (R1 <~> R2) by (eapply per_ctx_env_left_irrel; [apply H1 | apply H2]) || tactic_error R1 R2 *)
+(*         end *)
+(*     | H1 : {{ DF ^?Γ ≈ ^_ ∈ per_ctx_env ↘ ?R1 }}, *)
+(*         H2 : {{ DF ^_ ≈ ^?Γ ∈ per_ctx_env ↘ ?R2 }} |- _ => *)
+(*         (** Order matters less here as H1 and H2 cannot be exchanged *) *)
+(*         assert_fails (unify R1 R2); *)
+(*         match goal with *)
+(*         | H : R1 <~> R2 |- _ => fail 1 *)
+(*         | H : R2 <~> R1 |- _ => fail 1 *)
+(*         | _ => assert (R1 <~> R2) by (eapply per_ctx_env_cross_irrel; [apply H1 | apply H2]) || tactic_error R1 R2 *)
+(*         end *)
+(*     end. *)
+
+(* Ltac do_per_ctx_env_irrel_assert := *)
+(*   repeat do_per_ctx_env_irrel_assert1. *)
+
+(* Ltac handle_per_ctx_env_irrel := *)
+(*   functional_eval_rewrite_clear; *)
+(*   do_per_ctx_env_irrel_assert; *)
+(*   apply_relation_equivalence; *)
+(*   clear_dups. *)
+
+(* Lemma per_ctx_env_trans {P : PtsSig} {pred_P : PredicativeSig P} : forall Γ1 Γ2 R, *)
+(*     {{ DF Γ1 ≈ Γ2 ∈ @per_ctx_env P pred_P ↘ R }} -> *)
+(*     (forall Γ3, *)
+(*         {{ DF Γ2 ≈ Γ3 ∈ @per_ctx_env P pred_P ↘ R }} -> *)
+(*         {{ DF Γ1 ≈ Γ3 ∈ @per_ctx_env P pred_P ↘ R }}) /\ *)
+(*       (forall ρ1 ρ2 ρ3, *)
+(*           {{ Dom ρ1 ≈ ρ2 ∈ R }} -> *)
+(*           {{ Dom ρ2 ≈ ρ3 ∈ R }} -> *)
+(*           {{ Dom ρ1 ≈ ρ3 ∈ R }}). *)
+(* Proof with solve [eauto using per_sort_trans]. *)
+(*   simpl. *)
+(*   (* induction 1; subst; *) *)
+(*   (*   [> split; *) *)
+(*   (*    [ inversion 1; subst; eauto *) *)
+(*   (*    | intros; destruct_conjs; eauto] ..]; *) *)
+(*   (*   pose proof (@relation_equivalence_pointwise env); *) *)
+(*   (*   handle_per_ctx_env_irrel; *) *)
+(*   (*   try solve [intuition]. *) *)
+(*   (* - econstructor; only 4: reflexivity; eauto. *) *)
+(*   (*   + apply_relation_equivalence. intuition. *) *)
+(*   (*   + intros. *) *)
+(*   (*     assert (tail_rel ρ ρ) by intuition. *) *)
+(*   (*     assert (tail_rel0 ρ ρ') by intuition. *) *)
+(*   (*     destruct_rel_typ. *) *)
+(*   (*     handle_per_sort_elem_irrel. *) *)
+(*   (*     econstructor; intuition. *) *)
+(*   (*     (** This one cannot be replaced with `etransitivity` as we need different `i`s. *) *) *)
+(*   (*     eapply per_sort_trans; [| eassumption]; eassumption. *) *)
+(*   (* - destruct_by_head cons_per_ctx_env. *) *)
+(*   (*   assert (tail_rel d{{{ ρ ↯ }}} d{{{ ρ' ↯ }}}) by eauto. *) *)
+(*   (*   destruct_rel_typ. *) *)
+(*   (*   handle_per_sort_elem_irrel. *) *)
+(*   (*   eexists. *) *)
+(*   (*   apply_relation_equivalence. *) *)
+(*   (*   etransitivity; intuition. *) *)
+(* Admitted. *)
+
+(* Corollary per_ctx_trans {P : PtsSig} {pred_P : PredicativeSig P} : forall Γ1 Γ2 Γ3 R, *)
+(*     {{ DF Γ1 ≈ Γ2 ∈ @per_ctx_env P pred_P ↘ R }} -> *)
+(*     {{ DF Γ2 ≈ Γ3 ∈ @per_ctx_env P pred_P ↘ R }} -> *)
+(*     {{ DF Γ1 ≈ Γ3 ∈ @per_ctx_env P pred_P ↘ R }}. *)
+(* Proof. *)
+(*   intros * ?% per_ctx_env_trans. *)
+(*   firstorder. *)
+(* Qed. *)
+
+(* Corollary per_env_trans {P : PtsSig} {pred_P : PredicativeSig P} : forall Γ1 Γ2 R ρ1 ρ2 ρ3, *)
+(*     {{ DF Γ1 ≈ Γ2 ∈ @per_ctx_env P pred_P ↘ R }} -> *)
+(*     {{ Dom ρ1 ≈ ρ2 ∈ R }} -> *)
+(*     {{ Dom ρ2 ≈ ρ3 ∈ R }} -> *)
+(*     {{ Dom ρ1 ≈ ρ3 ∈ R }}. *)
+(* Proof. *)
+(*   intros * ?% per_ctx_env_trans. *)
+(*   firstorder. *)
+(* Qed. *)
+
+(* #[export] *)
+(* Instance per_ctx_PER {P : PtsSig} {pred_P : PredicativeSig P} {R} : PER (@per_ctx_env P pred_P R). *)
+(* Proof. *)
+(*   split. *)
+(*   - auto using per_ctx_sym. *)
+(*   - eauto using per_ctx_trans. *)
+(* Qed. *)
+
+(* #[export] *)
+(* Instance per_env_PER {P : PtsSig} {pred_P : PredicativeSig P} {R Γ Δ} (H : @per_ctx_env P pred_P R Γ Δ) : PER R. *)
+(* Proof. *)
+(*   split. *)
+(*   - pose proof (fun ρ ρ' => per_env_sym _ _ _ ρ ρ' H); auto. *)
+(*   - pose proof (fun ρ0 ρ1 ρ2 => per_env_trans _ _ _ ρ0 ρ1 ρ2 H); eauto. *)
+(* Qed. *)
+
+(* (** This lemma removes the PER argument *) *)
+(* Lemma per_ctx_env_cons' {P : PtsSig} {pred_P : PredicativeSig P} : forall {Γ Γ' s A A' tail_rel} *)
+(*                              (head_rel : forall {ρ ρ'} (equiv_ρ_ρ' : {{ Dom ρ ≈ ρ' ∈ tail_rel }}), relation (domain P)) *)
+(*                              env_rel, *)
+(*     {{ EF Γ ≈ Γ' ∈ @per_ctx_env P pred_P ↘ tail_rel }} -> *)
+(*     (forall {ρ ρ'} (equiv_ρ_ρ' : {{ Dom ρ ≈ ρ' ∈ tail_rel }}), *)
+(*         rel_typ pred_P s A ρ A' ρ' (head_rel equiv_ρ_ρ')) -> *)
+(*     (env_rel <~> cons_per_ctx_env tail_rel (@head_rel)) -> *)
+(*     {{ EF Γ, A::Sort@s ≈ Γ', A'::Sort@s ∈ @per_ctx_env P pred_P ↘ env_rel }}. *)
+(* Proof. *)
+(*   intros. *)
+(*   econstructor; eauto. *)
+(*   typeclasses eauto. *)
+(* Qed. *)
+
+(* #[export] *)
+(* Hint Resolve per_ctx_env_cons' : mcpts. *)
+
+(* Ltac per_ctx_env_econstructor := *)
+(*   (repeat intro; hnf; eapply per_ctx_env_cons') + econstructor. *)
+
+(* Lemma per_ctx_env_cons_clean_inversion {P : PtsSig} {pred_P : PredicativeSig P} : forall {Γ Γ' env_relΓ A A' env_relΓA s}, *)
+(*     {{ EF Γ ≈ Γ' ∈ @per_ctx_env P pred_P ↘ env_relΓ }} -> *)
+(*     {{ EF Γ, A::Sort@s ≈ Γ', A'::Sort@s ∈ @per_ctx_env P pred_P ↘ env_relΓA }} ->  *)
+(*     exists (head_rel : forall {ρ ρ'} (equiv_ρ_ρ' : {{ Dom ρ ≈ ρ' ∈ env_relΓ }}), relation (domain P)), *)
+(*       (forall ρ ρ' (equiv_ρ_ρ' : {{ Dom ρ ≈ ρ' ∈ env_relΓ }}), *)
+(*           rel_typ pred_P s A ρ A' ρ' (head_rel equiv_ρ_ρ')) /\ *)
+(*         (env_relΓA <~> cons_per_ctx_env env_relΓ (@head_rel)). *)
+(* Proof with intuition. *)
+(*   intros * HΓ HΓA. *)
+(*   inversion HΓA; subst. *)
+(*   handle_per_ctx_env_irrel. *)
+(*   eexists. *)
+(*   split; intros. *)
+(*   - instantiate (1 := fun ρ ρ' (equiv_ρ_ρ' : env_relΓ ρ ρ') m m' => *)
+(*                         forall R, *)
+(*                           rel_typ pred_P s A ρ A' ρ' R -> *)
+(*                           {{ Dom m ≈ m' ∈ R }}). *)
+(*     assert (tail_rel ρ ρ') by intuition. *)
+(*     (on_all_hyp: destruct_rel_by_assumption tail_rel). *)
+(*     econstructor; eauto. *)
+(*     apply -> per_sort_elem_morphism_iff; eauto. *)
+(*     split; intros... *)
+(*     destruct_by_head (@rel_typ P). *)
+(*     handle_per_sort_elem_irrel... *)
+(*   - intros ρ ρ'. *)
+(*     split; intros; destruct_by_head (@cons_per_ctx_env P); *)
+(*       assert {{ Dom ρ ↯ ≈ ρ' ↯ ∈ tail_rel }} by intuition; *)
+(*       (on_all_hyp: destruct_rel_by_assumption tail_rel); *)
+(*       unshelve eexists; intros... *)
+(*     destruct_by_head (@rel_typ P). *)
+(*     handle_per_sort_elem_irrel... *)
+    
+(* Admitted. *)
+
+(* Ltac invert_per_ctx_env H := *)
+(*   (unshelve eapply (per_ctx_env_cons_clean_inversion _) in H; [eassumption | |]; deex_in H; destruct H as []) *)
+(*   + (inversion H; subst). *)
+
+(* Ltac invert_per_ctx_envs := match_by_head per_ctx_env ltac:(fun H => directed invert_per_ctx_env H). *)
+
+(* Ltac invert_per_ctx_envs_of rel := match_by_head (per_ctx_env rel) ltac:(fun H => directed invert_per_ctx_env H). *)
+
+(* Lemma per_ctx_respects_length {P : PtsSig} {pred_P : PredicativeSig P} : forall {Γ Γ'}, *)
+(*     {{ Exp Γ ≈ Γ' ∈ @per_ctx P pred_P }} -> *)
+(*     length Γ = length Γ'. *)
+(* Proof. *)
+(*   intros * [? H]. *)
+(*   induction H; simpl; congruence. *)
+(* Qed. *)
+
+(* (* The remaining lemmas are about context subtyping.  We might need to replace them at some point *) *)
+
+(* (* Lemma per_ctx_subtyp_to_env : forall Γ Δ, *) *)
+(* (*     {{ SubE Γ <: Δ }} -> *) *)
+(* (*     exists R R', *) *)
+(* (*       {{ EF Γ ≈ Γ ∈ per_ctx_env ↘ R }} /\ *) *)
+(* (*         {{ EF Δ ≈ Δ ∈ per_ctx_env ↘ R' }}. *) *)
+(* (* Proof. *) *)
+(* (*   destruct 1; destruct_all. *) *)
+(* (*   - repeat eexists; econstructor; apply Equivalence_Reflexive. *) *)
+(* (*   - eauto. *) *)
+(* (* Qed. *) *)
+
+(* (* Lemma per_ctx_env_subtyping : forall Γ Δ, *) *)
+(* (*     {{ SubE Γ <: Δ }} -> *) *)
+(* (*     forall R R' ρ ρ', *) *)
+(* (*       {{ EF Γ ≈ Γ ∈ per_ctx_env ↘ R }} -> *) *)
+(* (*       {{ EF Δ ≈ Δ ∈ per_ctx_env ↘ R' }} -> *) *)
+(* (*       R ρ ρ' -> *) *)
+(* (*       R' ρ ρ'. *) *)
+(* (* Proof. *) *)
+(* (*   induction 1; intros; *) *)
+(* (*     handle_per_ctx_env_irrel; *) *)
+(* (*     invert_per_ctx_envs; *) *)
+(* (*     apply_relation_equivalence; *) *)
+(* (*     trivial. *) *)
+
+(* (*   destruct_by_head cons_per_ctx_env. *) *)
+(* (*   assert {{ Dom ρ ↯ ≈ ρ' ↯ ∈ tail_rel0 }} by intuition. *) *)
+(* (*   unshelve eexists; [eassumption |]. *) *)
+(* (*   destruct_rel_typ. *) *)
+(* (*   eapply per_elem_subtyping with (i := max i1 (max i0 i)); try eassumption. *) *)
+(* (*   - eauto using per_subtyp_cumu_right. *) *)
+(* (*   - saturate_refl. *) *)
+(* (*     eauto using per_sort_elem_cumu_max_left. *) *)
+(* (*   - saturate_refl. *) *)
+(* (*     eauto using per_sort_elem_cumu_max_left, per_sort_elem_cumu_max_right. *) *)
+(* (* Qed. *) *)
+
+(* (* Lemma per_ctx_subtyp_refl1 : forall Γ Δ R, *) *)
+(* (*     {{ EF Γ ≈ Δ ∈ per_ctx_env ↘ R }} -> *) *)
+(* (*     {{ SubE Γ <: Δ }}. *) *)
+(* (* Proof. *) *)
+(* (*   induction 1; mauto. *) *)
+
+(* (*   assert (exists R, {{ EF Γ , A ≈ Γ' , A' ∈ per_ctx_env ↘ R }}) by *) *)
+(* (*     (eexists; eapply per_ctx_env_cons'; eassumption). *) *)
+(* (*   destruct_all. *) *)
+(* (*   econstructor; try solve [saturate_refl; mauto 2]. *) *)
+(* (*   intros. *) *)
+(* (*   destruct_rel_typ. *) *)
+(* (*   simplify_evals. *) *)
+(* (*   eauto using per_subtyp_refl1. *) *)
+(* (* Qed. *) *)
+
+(* (* Lemma per_ctx_subtyp_refl2 : forall Γ Δ R, *) *)
+(* (*     {{ EF Γ ≈ Δ ∈ per_ctx_env ↘ R }} -> *) *)
+(* (*     {{ SubE Δ <: Γ }}. *) *)
+(* (* Proof. *) *)
+(* (*   intros. symmetry in H. eauto using per_ctx_subtyp_refl1. *) *)
+(* (* Qed. *) *)
+
+(* (* Lemma per_ctx_subtyp_trans : forall Γ1 Γ2, *) *)
+(* (*     {{ SubE Γ1 <: Γ2 }} -> *) *)
+(* (*     forall Γ3, *) *)
+(* (*       {{ SubE Γ2 <: Γ3 }} -> *) *)
+(* (*       {{ SubE Γ1 <: Γ3 }}. *) *)
+(* (* Proof. *) *)
+(* (*   induction 1; intros; *) *)
+(* (*     dir_inversion_by_head per_ctx_subtyp; subst; *) *)
+(* (*     repeat invert_per_ctx_envs; *) *)
+(* (*     mauto 1; clear_PER. *) *)
+
+(* (*   handle_per_ctx_env_irrel. *) *)
+(* (*   econstructor; try eassumption. *) *)
+(* (*   - firstorder. *) *)
+(* (*   - instantiate (1 := max i i0). *) *)
+(* (*     intros. *) *)
+(* (*     assert {{ Dom ρ ≈ ρ' ∈ tail_rel0 }} *) *)
+(* (*       by (apply_relation_equivalence; eapply per_ctx_env_subtyping; revgoals; eassumption). *) *)
+(* (*     saturate_refl_for tail_rel. *) *)
+(* (*     destruct_rel_typ. *) *)
+(* (*     handle_per_sort_elem_irrel. *) *)
+(* (*     etransitivity; intuition mauto using per_subtyp_cumu_left, per_subtyp_cumu_right. *) *)
+(* (*   - econstructor; intuition. *) *)
+(* (*     + typeclasses eauto. *) *)
+(* (*     + solve_refl. *) *)
+(* (*   - econstructor; mauto 3. *) *)
+(* (*     + typeclasses eauto. *) *)
+(* (*     + solve_refl. *) *)
+(* (* Qed. *) *)
+
+(* (* #[export] *) *)
+(* (* Hint Resolve per_ctx_subtyp_trans : mcpts. *) *)
+
+(* (* #[export] *) *)
+(* (* Instance per_ctx_subtyp_trans_ins : Transitive per_ctx_subtyp. *) *)
+(* (* Proof. *) *)
+(* (*   eauto using per_ctx_subtyp_trans. *) *)
+(* (* Qed. *) *)
